Iris proof mode instance

theories/Predicates.v
@@ -31,6 +31,9 @@ From Coq Require Import
   Classes.Morphisms_Prop
   Classes.RelationClasses
   Relations.Relation_Definitions.
+From iris Require
+  bi.derived_connectives
+  bi.interface.
 From Em Require Import
   Context
   Definitions
@@ -45,7 +48,6 @@ Set Implicit Arguments.
 #[local] Arguments Ty_func {Σ}.
 
 Module Pred.
-  Import World.notations.
   #[local] Notation Expr := (Sem expr).
 
   Declare Scope pred_scope.
@@ -57,59 +59,59 @@ Module Pred.
 
   Section RewriteRelations.
 
+    Import iris.bi.interface.
+
     Context {w : World}.
 
-    Definition bientails : relation (Pred w) :=
-      fun P Q => forall ι, P ι <-> Q ι.
-    Definition entails : relation (Pred w) :=
-      fun P Q => forall ι, P ι -> Q ι.
+    Record bientails (P Q : Pred w) : Prop :=
+      MkBientails
+        { fromBientails : forall ι, P ι <-> Q ι }.
+    Record entails (P Q : Pred w) : Prop :=
+      MkEntails
+        { fromEntails : forall ι, P ι -> Q ι }.
 
-    #[export] Instance equivalence_bientails : Equivalence bientails.
-    Proof.
-      constructor; unfold Reflexive, Symmetric, Transitive, bientails;
-        [ reflexivity | now symmetry | now etransitivity ].
-    Qed.
+    #[export] Instance pred_equiv : Equiv (Pred w) := bientails.
+    #[export] Instance pred_equivalence : Equivalence (≡@{Pred w}).
+    Proof. firstorder. Qed.
+
     #[export] Instance preorder_entails : RelationClasses.PreOrder entails.
-    Proof. constructor; unfold Reflexive, Transitive, entails; auto. Qed.
-
+    Proof. firstorder. Qed.
     #[export] Instance subrelation_bientails_entails :
-      subrelation bientails entails.
-    Proof. intros x y xy ι. apply xy. Qed.
-
+      subrelation (≡@{Pred w}) entails.
+    Proof. firstorder. Qed.
     #[export] Instance subrelation_bientails_flip_entails :
-      subrelation bientails (Basics.flip entails).
-    Proof. intros x y xy ι. apply xy. Qed.
+      subrelation (≡@{Pred w}) (Basics.flip entails).
+    Proof. firstorder. Qed.
 
     (* #[export] Instance proper_bientails : *)
     (*   Proper (bientails ==> bientails ==> iff) bientails. *)
     (* Proof. intuition. Qed. *)
     #[export] Instance proper_entails_bientails :
-      Proper (bientails ==> bientails ==> iff) entails.
-    Proof. unfold Proper, respectful, bientails, entails. intuition. Qed.
+      Proper ((≡@{Pred w}) ==> (≡@{Pred w}) ==> iff) entails.
+    Proof. firstorder. Qed.
     #[export] Instance proper_entails_entails :
       Proper (Basics.flip entails ==> entails ==> Basics.impl) entails.
-    Proof. unfold Proper, respectful, Basics.impl, entails. intuition. Qed.
+    Proof. firstorder. Qed.
 
   End RewriteRelations.
   #[global] Arguments bientails {w} (_ _)%P.
   #[global] Arguments entails {w} (_ _)%P.
-  #[global] Typeclasses Opaque entails.
-  #[global] Typeclasses Opaque bientails.
 
   Section Definitions.
+    Import World.notations.
 
-    Definition Falseₚ : ⊢ Pred :=
+    Definition Falseₚ : ⊢ʷ Pred :=
       fun w _ => Logic.False.
-    Definition Trueₚ : ⊢ Pred :=
+    Definition Trueₚ : ⊢ʷ Pred :=
       fun w _ => Logic.True.
-    Definition iffₚ : ⊢ Pred -> Pred -> Pred :=
+    Definition iffₚ : ⊢ʷ Pred -> Pred -> Pred :=
       fun w P Q ι => P ι <-> Q ι.
-    Definition implₚ : ⊢ Pred -> Pred -> Pred :=
-      fun w P Q ι => (P ι -> Q ι)%type.
-    Definition andₚ : ⊢ Pred -> Pred -> Pred :=
-      fun w P Q ι => (P ι /\ Q ι)%type.
-    Definition orₚ : ⊢ Pred -> Pred -> Pred :=
-      fun w P Q ι => (P ι \/ Q ι)%type.
+    Definition implₚ : ⊢ʷ Pred -> Pred -> Pred :=
+      fun w P Q ι => P ι -> Q ι.
+    Definition andₚ : ⊢ʷ Pred -> Pred -> Pred :=
+      fun w P Q ι => P ι /\ Q ι.
+    Definition orₚ : ⊢ʷ Pred -> Pred -> Pred :=
+      fun w P Q ι => P ι \/ Q ι.
     #[global] Arguments andₚ {_} (_ _)%P _/.
     #[global] Arguments orₚ {_} (_ _)%P _/.
     #[global] Arguments iffₚ {_} (_ _)%P _/.
@@ -118,126 +120,219 @@ Module Pred.
     #[global] Arguments Falseₚ {_} _/.
 
     Definition eqₚ {T : TYPE} {A : Type} {instTA : Inst T A} :
-      ⊢ T -> T -> Pred :=
+      ⊢ʷ T -> T -> Pred :=
       fun w t1 t2 ι => inst t1 ι = inst t2 ι.
     #[global] Arguments eqₚ {T A _} [w] _ _ _/.
 
-
-    Polymorphic Definition Forall {I : Type} {w} : (I -> Pred w) -> Pred w :=
-      fun A ι => forall i : I, A i ι.
-    Polymorphic Definition Exists {I : Type} {w} : (I -> Pred w) -> Pred w :=
-      fun A ι => exists i : I, A i ι.
+    (* #[universes(polymorphic)]  *)Definition Forall {I : Type} {w} :
+      (I -> Pred w) -> Pred w := fun A ι => forall i : I, A i ι.
+    (* #[universes(polymorphic)]  *)Definition Exists {I : Type} {w} :
+      (I -> Pred w) -> Pred w := fun A ι => exists i : I, A i ι.
     #[global] Arguments Forall {I w} A%P ι/.
     #[global] Arguments Exists {I w} A%P ι/.
 
     Definition Ext {R : ACC} {instR : forall w, Inst (R w) (Assignment w)} :
-      ⊢ Pred -> Box R Pred :=
-      fun w0 p w1 r ι => p (inst r ι).
-    #[global] Arguments Ext {_ _} [w] _%P [_] _ _/.
+      ⊢ʷ Pred -> Box R Pred := fun w0 p w1 r ι => p (inst r ι).
+    #[global] Arguments Ext {_ _} [w] _%P [_] _ ι/.
     #[global] Instance params_ext : Params (@Ext) 6 := {}.
 
-    Definition TPB : ⊢ Env -> Const expr -> Ty -> Expr -> Pred :=
+    Definition TPB : ⊢ʷ Env -> Const expr -> Ty -> Expr -> Pred :=
       fun w G e t ee ι => inst G ι |-- e ; inst t ι ~> inst ee ι.
     #[global] Arguments TPB [w] G e t ee ι/.
 
+    (* Definition TPB {w : World} (G : Env w) (e : expr) (t : Ty w) (ee : Expr w) : Pred w := *)
+    (*   fun ι => inst G ι |-- e ; inst t ι ~> inst ee ι. *)
+    (* #[global] Arguments TPB [w] G e t ee ι/. *)
+
   End Definitions.
+
+  Module Import proofmode.
+
+    Import iris.bi.interface.
+
+    Variant empₚ {w} (ι : Assignment w) : Prop :=
+      MkEmp : empₚ ι.
+    Variant sepₚ {w} (P Q : Pred w) (ι : Assignment w) : Prop :=
+      MkSep : P ι -> Q ι -> sepₚ P Q ι.
+    Variant wandₚ {w} (P Q : Pred w) (ι : Assignment w) : Prop :=
+      MkWand : (P ι -> Q ι) -> wandₚ P Q ι.
+    Variant persistently {w} (P : Pred w) (ι : Assignment w) : Prop :=
+      MkPersistently : P ι -> persistently P ι.
+
+    #[export] Instance ofe_dist_pred {w} : ofe.Dist (Pred w) :=
+      ofe.discrete_dist.
+
+    Definition bimixin_pred {w : World} :
+      BiMixin entails empₚ (fun P _ => P) andₚ orₚ implₚ
+        (fun A => @Pred.Forall A w) (fun A => @Pred.Exists A w)
+        sepₚ wandₚ persistently.
+    Proof. firstorder. Qed.
+
+    (* Iris defines [bi_later_mixin_id] for BI algebras without later. However,
+       the identity function as later still causes some later-specific
+       typeclasses to be picked. We just define our own trivial modality and
+       mixin to avoid that. *)
+    Variant later {w} (P : Pred w) (ι : Assignment w) : Prop :=
+      MkLater : P ι -> later P ι.
+
+    Definition bilatermixin_pred {w} :
+      BiLaterMixin entails (fun P _ => P) orₚ implₚ
+        (fun A => @Pred.Forall A w) (fun A => @Pred.Exists A w)
+        sepₚ persistently later.
+    Proof. firstorder. Qed.
+
+    Canonical bi_pred {w : World} : bi :=
+      {| bi_car            := Pred w;
+         bi_cofe           := ofe.discrete_cofe _;
+         bi_bi_mixin       := bimixin_pred;
+         bi_bi_later_mixin := bilatermixin_pred;
+      |}.
+
+    #[export] Instance persistent_pred {w} {P : Pred w} :
+      derived_connectives.Persistent P.
+    Proof. constructor. intros ι HP. constructor. exact HP. Qed.
+
+    #[export] Instance affine_pred {w} {P : Pred w} :
+      derived_connectives.Affine P.
+    Proof. constructor. intros ι HP. constructor. Qed.
+
+  End proofmode.
 
   Module Import notations.
 
-    Infix "⊣⊢ₚ" := (bientails) (at level 95).
+    Import iris.bi.interface.
+    Import iris.bi.derived_connectives.
+
+    Notation "P ⊣⊢ₚ Q" :=
+      (@equiv (bi_car (@bi_pred _)) (@pred_equiv _) P%P Q%P)
+        (at level 95).
+    Notation "(⊣⊢ₚ)" :=
+      (@equiv (bi_car (@bi_pred _)) (@pred_equiv _))
+        (only parsing).
+
     Infix "⊢ₚ" := (entails) (at level 95).
 
-    Notation "⊤ₚ" := Trueₚ : pred_scope.
-    Notation "⊥ₚ" := Falseₚ : pred_scope.
-    Infix "<->ₚ"  := (iffₚ) (at level 94) : pred_scope.
-    Infix "->ₚ"   := (implₚ) (at level 94, right associativity) : pred_scope.
-    Infix "/\ₚ"   := (andₚ) (at level 80, right associativity) : pred_scope.
-    Infix "\/ₚ"   := (orₚ) (at level 85, right associativity) : pred_scope.
+    Notation "⊤ₚ" := (@bi_pure (@bi_pred _) True) : pred_scope.
+    Notation "⊥ₚ" := (@bi_pure (@bi_pred _) False) : pred_scope.
+    Notation "P <->ₚ Q" := (@bi_iff (@bi_pred _) P%P Q%P) (at level 94) : pred_scope.
+    Notation "P ->ₚ Q"  := (@bi_impl (@bi_pred _) P%P Q%P) (at level 94, right associativity) : pred_scope.
+    Notation "P /\ₚ Q"  := (@bi_and (@bi_pred _) P%P Q%P) (at level 80, right associativity) : pred_scope.
+    Notation "P \/ₚ Q"  := (@bi_or (@bi_pred _) P%P Q%P) (at level 85, right associativity) : pred_scope.
 
     Infix "=ₚ" := eqₚ (at level 70, no associativity) : pred_scope.
 
-    Notation "'∀ₚ' x ∶ T , Q" :=
-      (@Forall T _ (fun x => Q%P))
-        (at level 99, x binder, x at next level, T at level 95,
-          right associativity,
-          format "'∀ₚ'  x  ∶  T ,  Q")
-      : pred_scope.
-
-    Notation "'∀ₚ⁺' x .. y , Q " :=
-      (Forall (fun x => .. (Forall (fun y => Q%P)) ..))
-        (at level 99, x binder, y binder, right associativity,
-        only parsing)
-      : pred_scope.
-
-    (* Notation "'∃' x .. y , Q " := *)
-    (*     (Exists (fun x => .. (Exists (fun y => Q%P)) ..)) *)
-    (*       (at level 94, x binder, y binder, right associativity) *)
-    (*     : pred_scope. *)
-
-    Notation "'∃ₚ' x ∶ T , Q" :=
-      (@Exists T _ (fun x => Q%P))
-        (at level 99, x binder, right associativity,
-          format "'∃ₚ'  x  ∶  T ,  Q")
-        : pred_scope.
+    Notation "∀ₚ x .. y , P" :=
+      (@bi_forall (@bi_pred _) _ (fun x => .. (@bi_forall (@bi_pred _) _ (fun y => P%P)) ..))
+      (at level 200, x binder, y binder, right associativity,
+        format "'[ ' '[ ' ∀ₚ  x .. y ']' ,  '/' P ']'") : pred_scope.
+    Notation "∃ₚ x .. y , P" :=
+      (@bi_exist (@bi_pred _) _ (fun x => .. (@bi_exist (@bi_pred _) _ (fun y => P%P)) ..))
+      (at level 200, x binder, y binder, right associativity,
+        format "'[ ' '[ ' ∃ₚ  x .. y ']' ,  '/' P ']'") : pred_scope.
 
     Notation "'Fun' x => b" :=
       (fun w ζ x => b%P w ζ)
-        (x binder, at level 100) : pred_scope.
+        (x binder, at level 100, only parsing) : pred_scope.
 
     Notation "G |--ₚ E ; T ~> EE" :=
       (TPB G E T EE) (at level 70, no associativity) : pred_scope.
 
   End notations.
 
+  Ltac pred_unfold :=
+    repeat
+      (change (@interface.bi_and (@bi_pred ?w)) with (@andₚ w) in *;
+       change (@interface.bi_or (@bi_pred ?w)) with (@orₚ w) in *;
+       change (@interface.bi_impl (@bi_pred ?w)) with (@implₚ w) in *;
+       change (@derived_connectives.bi_iff (@bi_pred ?w)) with (@iffₚ w) in *;
+       change (@interface.bi_pure (@bi_pred ?w)) with (fun (P : Prop) (ι : Assignment w) => P) in *;
+       change (@interface.bi_forall (@bi_pred ?w)) with (fun A => @Forall A w) in *;
+       change (@interface.bi_exist (@bi_pred ?w)) with (fun A => @Exists A w) in *;
+       cbn [andₚ orₚ implₚ iffₚ Forall Exists Ext eqₚ TPB inst inst_ty inst_env] in *
+      );
+    rewrite ?inst_persist, ?inst_lift in *;
+    repeat
+      match goal with
+      | H: context[@inst ?AT ?A ?I ?w ?x ?ι] |- _ =>
+          is_var x; generalize dependent x; intro x;
+          generalize (@inst AT A I w x ι);
+          clear x; intro x; intros; subst
+      | |- context[@inst ?AT ?A ?I ?w ?x ?ι] =>
+          is_var x; generalize dependent x; intro x;
+          generalize (@inst AT A I w x ι);
+          clear x; intro x; intros; subst
+      end.
+
   Definition ProperPost {R} {reflR : Refl R} {instR : forall w : World, Inst (R w) (Assignment w)}
-    {AT A} {persA : Persistent R AT} {instT : Inst AT A}
-    {w} (Q : Box R (AT -> Pred) w) : Prop :=
+    {AT A} {persA : Definitions.Persistent R AT} {instT : Inst AT A}
+    {w} (Q : Box R (Impl AT Pred) w) : Prop :=
     forall w1 (r01 : R w w1) (te0 : AT w) (te1 : AT w1),
       (te1 =ₚ (persist _ te0 _ r01)) ⊢ₚ (Ext (Q w refl te0) r01 <->ₚ Q w1 r01 te1).
 
   Section Lemmas.
 
+    Import iris.bi.interface.
+    Import stdpp.base.
+
     Create HintDb obligation.
     #[local] Hint Rewrite @inst_refl @inst_trans : obligation.
 
     #[local] Ltac obligation :=
-      unfold Proper, respectful, pointwise_relation, forall_relation,
-        entails, bientails;
-        cbn; intros; subst;
-      try (match goal with
+      cbv [Proper flip respectful pointwise_relation forall_relation];
+      repeat (autorewrite with obligation in *; cbn in *; intros; subst; pred_unfold);
+      repeat
+        (match goal with
+         (* | H: _ ⊢ₚ _ |- _ => destruct H as [H] *)
+         (* | H: _ ⊣⊢ₚ _ |- _ => destruct H as [H] *)
+         | H: forall (H : ?A), _, a : ?A |- _ =>
+           specialize (H a); autorewrite with obligation in H; cbn in H
          | |- (forall _ : ?A, _) <-> (forall _ : ?A, _) =>
-             apply all_iff_morphism; intro
+             apply all_iff_morphism; intro; autorewrite with obligation; cbn
          | |- (exists _ : ?A, _) <-> (exists _ : ?A, _) =>
-             apply ex_iff_morphism; intro
+             apply ex_iff_morphism; intro; autorewrite with obligation; cbn
+         (* | |- _ ⊣⊢ₚ _ => constructor; cbn; intros *)
+         (* | |- _ ⊢ₚ _ => constructor; cbn; intros *)
          end);
-      autorewrite with obligation;
       try easy; try (intuition; fail); try (intuition congruence; fail).
     #[local] Obligation Tactic := obligation.
 
+    Lemma entails_in [w] (P Q : Pred w) :
+      (P ⊢ₚ Q) <-> forall ι, P ι -> Q ι.
+    Proof. split; [intros []|]; obligation. Qed.
+    Lemma equiv_in [w] (P Q : Pred w) :
+      (P ⊣⊢ₚ Q) <-> forall ι, P ι <-> Q ι.
+    Proof. split; [intros []|]; obligation. Qed.
+
+    #[local] Hint Rewrite entails_in equiv_in : obligation.
+    #[local] Hint Rewrite <- @Prelude.forall_and_compat : obligation.
+
     #[export,program] Instance proper_iff {w} :
-      Proper (bientails ==> bientails ==> bientails) (@iffₚ w).
+      Proper ((⊣⊢ₚ) ==> (⊣⊢ₚ) ==> (⊣⊢ₚ)) (@iffₚ w).
     #[export,program] Instance proper_impl_bientails {w} :
-      Proper (bientails ==> bientails ==> bientails) (@implₚ w).
+      Proper ((⊣⊢ₚ) ==> (⊣⊢ₚ) ==> (⊣⊢ₚ)) (@implₚ w).
     #[export,program] Instance proper_impl_entails {w} :
       Proper (entails --> entails ==> entails) (@implₚ w).
     #[export,program] Instance proper_and_bientails {w} :
-      Proper (bientails ==> bientails ==> bientails) (@andₚ w).
+      Proper ((⊣⊢ₚ) ==> (⊣⊢ₚ) ==> (⊣⊢ₚ)) (@andₚ w).
     #[export,program] Instance proper_and_entails {w} :
       Proper (entails ==> entails ==> entails) (@andₚ w).
     #[export,program] Instance proper_or_bientails {w} :
-      Proper (bientails ==> bientails ==> bientails) (@orₚ w).
+      Proper ((⊣⊢ₚ) ==> (⊣⊢ₚ) ==> (⊣⊢ₚ)) (@orₚ w).
     #[export,program] Instance proper_or_entails {w} :
       Proper (entails ==> entails ==> entails) (@orₚ w).
     #[export,program] Instance proper_bientails_forall {I w} :
-      Proper (pointwise_relation I bientails ==> bientails) (@Forall I w).
+      Proper (pointwise_relation I (⊣⊢ₚ) ==> (⊣⊢ₚ)) (@Pred.Forall I w).
     #[export,program] Instance proper_bientails_exists {I w} :
-      Proper (pointwise_relation I bientails ==> bientails) (@Exists I w).
+      Proper (pointwise_relation I (⊣⊢ₚ) ==> (⊣⊢ₚ)) (@Pred.Exists I w).
     #[export,program] Instance proper_ext_bientails
       {R : ACC} {instR : forall w, Inst (R w) (Assignment w)} {w} :
-      Proper (bientails ==> forall_relation (fun _ => eq ==> bientails)) (Ext (R:=R) (w:=w)).
+      Proper ((⊣⊢ₚ) ==> forall_relation (fun _ => eq ==> (⊣⊢ₚ))) (Ext (R:=R) (w:=w)).
     #[export,program] Instance proper_ext_entails
       {R : ACC} {instR : forall w, Inst (R w) (Assignment w)} {w} :
       Proper (entails ==> forall_relation (fun _ => eq ==> entails)) (Ext (R:=R) (w:=w)).
+    #[export,program] Instance proper_ext_flip_entails
+      {R : ACC} {instR : forall w, Inst (R w) (Assignment w)} {w} :
+      Proper (entails --> forall_relation (fun _ => eq ==> Basics.flip entails)) (Ext (R:=R) (w:=w)).
 
     Lemma split_bientails {w} (P Q : Pred w) :
       (P ⊣⊢ₚ Q) <-> (P ⊢ₚ Q) /\ (Q ⊢ₚ P).
@@ -280,19 +375,21 @@ Module Pred.
     Proof. obligation. Qed.
     Lemma impl_forget {w} (P Q R : Pred w) : P ⊢ₚ R -> P ⊢ₚ (Q ->ₚ R).
     Proof. obligation. Qed.
-
-    Lemma forall_l {I : Type} {w} (P : I -> Pred w) Q :
-      (exists x : I, P x ⊢ₚ Q) -> (∀ₚ x ∶ I, P x) ⊢ₚ Q.
-    Proof. obligation. firstorder. Qed.
-    Lemma forall_r {I : Type} {w} P (Q : I -> Pred w) :
-      (P ⊢ₚ (∀ₚ x ∶ I, Q x)) <-> (forall x : I, P ⊢ₚ Q x).
+    Lemma impl_and [w] (P Q R : Pred w) : ((P /\ₚ Q) ->ₚ R) ⊣⊢ₚ (P ->ₚ Q ->ₚ R).
     Proof. obligation. Qed.
 
+    Lemma forall_l {I : Type} {w} (P : I -> Pred w) Q :
+      (exists x : I, P x ⊢ₚ Q) -> (∀ x : I, P x)%I ⊢ₚ Q.
+    Proof. obligation. firstorder. Qed.
+    Lemma forall_r {I : Type} {w} P (Q : I -> Pred w) :
+      (P ⊢ₚ (∀ₚ x : I, Q x)) <-> (forall x : I, P ⊢ₚ Q x).
+    Proof. obligation. firstorder. Qed.
+
     Lemma exists_l {I : Type} {w} (P : I -> Pred w) (Q : Pred w) :
-      (forall x : I, P x ⊢ₚ Q) -> (∃ₚ x ∶ I, P x) ⊢ₚ Q.
+      (forall x : I, P x ⊢ₚ Q) -> (∃ₚ x : I, P x) ⊢ₚ Q.
     Proof. obligation. firstorder. Qed.
     Lemma exists_r {I : Type} {w} P (Q : I -> Pred w) :
-      (exists x : I, P ⊢ₚ Q x) -> P ⊢ₚ (∃ₚ x ∶ I, Q x).
+      (exists x : I, P ⊢ₚ Q x) -> P ⊢ₚ (∃ₚ x : I, Q x).
     Proof. obligation. firstorder. Qed.
     #[global] Arguments exists_r {I w P Q} _.
 
@@ -331,11 +428,23 @@ Module Pred.
             end.
     Proof. destruct t1, t2; obligation. Qed.
 
+    Lemma eq_pair
+      {AT BT : TYPE} {A B : Type} {instA : Inst AT A} {instB : Inst BT B}
+      [w] (a1 a2 : AT w) (b1 b2 : BT w) :
+      (a1,b1) =ₚ (a2,b2) ⊣⊢ₚ ((a1 =ₚ a2) /\ₚ (b1 =ₚ b2)).
+    Proof.
+      constructor. pred_unfold. intros ι; cbn. split.
+      - now injection 1.
+      - intros []. now f_equal.
+    Qed.
+
     Section Ext.
+
+      Import World.notations.
 
       Context {R : ACC} {instR : forall w, Inst (R w) (Assignment w)}.
 
-      Lemma ext_refl {reflR : Refl R} {instReflR : InstRefl R} {w} (P : Pred w) :
+      Lemma ext_refl {reflR : Refl R} {instReflR : InstRefl R} [w] (P : Pred w) :
         Ext P refl ⊣⊢ₚ P.
       Proof. obligation. Qed.
       Lemma ext_trans {transR : Trans R}
@@ -354,49 +463,64 @@ Module Pred.
       Lemma ext_true {w0 w1} (ζ01 : R w0 w1) :
         Ext ⊤ₚ ζ01 ⊣⊢ₚ ⊤ₚ.
       Proof. obligation. Qed.
-      Lemma ext_eq {T : TYPE} {persR : Persistent R T}
+      Lemma ext_eq {T : TYPE} {persR : Definitions.Persistent R T}
         {A : Type} {instTA : Inst T A}
         {w0 w1} (r : R w0 w1) (t1 t2 : T w0) :
         Ext (t1 =ₚ t2) r ⊣⊢ₚ persist w0 t1 w1 r =ₚ persist w0 t2 w1 r.
       Proof.
-        unfold bientails, eqₚ, Ext. intros ι.
+        constructor. unfold eqₚ, Ext. intros ι.
         (* now rewrite !inst_persist. *)
       Admitted.
 
-      Polymorphic Lemma ext_forall {A} {w1 w2} (r12 : R w1 w2) (Q : A -> Pred w1) :
-        Ext (∀ₚ a ∶ A, Q a) r12 ⊣⊢ₚ (∀ₚ a ∶ A, Ext (Q a) r12).
+      (* #[universes(polymorphic)]  *)Lemma ext_forall [A] [w1 w2] (r12 : R w1 w2) (Q : A -> Pred w1) :
+        Ext (∀ₚ a : A, Q a) r12 ⊣⊢ₚ (∀ₚ a : A, Ext (Q a) r12).
       Proof. obligation. Qed.
-      Polymorphic Lemma ext_exists {A} {w1 w2} (r12 : R w1 w2) (Q : A -> Pred w1) :
-        Ext (∃ₚ a ∶ A, Q a) r12 ⊣⊢ₚ (∃ₚ a ∶ A, Ext (Q a) r12).
+      (* #[universes(polymorphic)]  *)Lemma ext_exists [A] [w1 w2] (r12 : R w1 w2) (Q : A -> Pred w1) :
+        Ext (∃ₚ a : A, Q a) r12 ⊣⊢ₚ (∃ₚ a : A, Ext (Q a) r12).
       Proof. obligation. Qed.
 
-      Lemma ext_tpb {persRTy : Persistent R Ty}
+      Import (hints) Sub.
+      Lemma ext_reduce  {w α} (t : Ty w) P Q :
+        (Ext P (step (R := Sub)) ⊢ₚ
+           Ty_hole ctx.in_zero =ₚ persist w t (ctx.snoc w α) (step (R := Sub)) ->ₚ Q) ->
+        P ⊢ₚ Ext Q (reduce (R := Sub) α t).
+      Proof.
+        rewrite ?entails_in. intros H ι HP. pred_unfold. rewrite inst_reduce.
+        specialize (H (env.snoc ι α (inst t ι))).
+        rewrite inst_persist inst_step_snoc in H. now apply H.
+      Qed.
+
+      Lemma ext_tpb {persRTy : Definitions.Persistent R Ty}
         {w1 w2} (r12 : R w1 w2) G (e : expr) (t : Ty w1) (ee : Expr w1) :
         Ext (G |--ₚ e; t ~> ee) r12 ⊣⊢ₚ
-        persist w1 G w2 r12 |--ₚ persist w1 e w2 r12; persist w1 t w2 r12 ~> persist w1 ee w2 r12.
-      Proof. obligation. now rewrite inst_persist_ty, inst_persist_env. Qed.
+        persist w1 G w2 r12 |--ₚ e; persist w1 t w2 r12 ~> persist w1 ee w2 r12.
+      Proof. obligation. Qed.
 
     End Ext.
 
   End Lemmas.
 
-  (* A type class for things that can be interpreted as a predicate. *)
-  Class InstPred (A : TYPE) :=
-    instpred : ⊢ A -> Pred.
+  Section InstPred.
+    Import World.notations.
+    (* A type class for things that can be interpreted as a predicate. *)
+    Class InstPred (A : TYPE) :=
+      instpred : ⊢ʷ A -> Pred.
 
-  #[export] Instance instpred_option {A} `{ipA : InstPred A} :
-    InstPred (Option A) :=
-    fun w o => match o with Some p => instpred p | None => Falseₚ end.
-  #[export] Instance instpred_list {A} `{ipA : InstPred A} :
-    InstPred (List A) :=
-    fun w =>
-      fix ip xs {struct xs} :=
-      match xs with
-      | nil       => Trueₚ
-      | cons y ys => andₚ (instpred y) (ip ys)
-      end.
+    #[export] Instance instpred_option {A} `{ipA : InstPred A} :
+      InstPred (Option A) :=
+      fun w o => match o with Some p => instpred p | None => Falseₚ end.
+    #[export] Instance instpred_list {A} `{ipA : InstPred A} :
+      InstPred (List A) :=
+      fun w =>
+        fix ip xs {struct xs} :=
+        match xs with
+        | nil       => Trueₚ
+        | cons y ys => andₚ (instpred y) (ip ys)
+        end.
+  End InstPred.
 
   Module Acc.
+    Import World.notations.
     Import (hints) Sub.
     Section WithAccessibilityRelation.
       Context {R : ACC} {instR : forall w, Inst (R w) (Assignment w)}.
@@ -406,38 +530,29 @@ Module Pred.
       Definition wlp {w0 w1} (r01 : R w0 w1) (Q : Pred w1) : Pred w0 :=
         fun ι0 => forall (ι1 : Assignment w1), inst r01 ι1 = ι0 -> Q ι1.
 
-      #[local] Arguments wp {_ _} _ _ _/.
-      #[local] Arguments wlp {_ _} _ _ _/.
+      #[global] Arguments wp {_ _} _ _ ι0/.
+      #[global] Arguments wlp {_ _} _ _ ι0/.
 
       #[export] Instance proper_wp_bientails {w0 w1} (r01 : R w0 w1) :
         Proper (bientails ==> bientails) (@wp w0 w1 r01).
-      Proof.
-        intros p q pq ι. cbn. apply ex_iff_morphism.
-        intros ι1. apply and_iff_morphism. easy. apply pq.
-      Qed.
+      Proof. firstorder. Qed.
 
       #[export] Instance proper_wp_entails {w0 w1} (r01 : R w0 w1) :
         Proper (entails ==> entails) (@wp w0 w1 r01).
-      Proof.
-        intros p q pq ι. cbn. intros (ι0 & Heq & HP).
-        exists ι0. split. easy. now apply pq.
-      Qed.
+      Proof. firstorder. Qed.
 
       #[export] Instance proper_wlp_bientails {w0 w1} (r01 : R w0 w1) :
         Proper (bientails ==> bientails) (@wlp w0 w1 r01).
-      Proof.
-        intros p q pq ι. cbn. apply all_iff_morphism. intros ι1.
-        now apply iff_iff_iff_impl_morphism.
-      Qed.
+      Proof. firstorder. Qed.
 
       #[export] Instance proper_wlp_entails {w0 w1} (r01 : R w0 w1) :
         Proper (entails ==> entails) (@wlp w0 w1 r01).
-      Proof. intros P Q HPQ ι HP ι0 Heq. now apply HPQ, HP. Qed.
+      Proof. firstorder. Qed.
 
       Lemma wp_refl {reflR : Refl R} {instReflR : InstRefl R}
         {w} (Q : Pred w) : wp refl Q ⊣⊢ₚ Q.
       Proof.
-        split; cbn.
+        constructor. split; cbn.
         - intros (ι' & Heq & HQ). rewrite inst_refl in Heq. now subst.
         - intros HQ. exists ι. split. now rewrite inst_refl. easy.
       Qed.
@@ -446,7 +561,7 @@ Module Pred.
         {w0 w1 w2} (r01 : R w0 w1) (r12 : R w1 w2) Q :
         wp (r01 ⊙ r12) Q ⊣⊢ₚ wp r01 (wp r12 Q).
       Proof.
-        split; cbn.
+        constructor. split; cbn.
         - intros (ι2 & Heq & HQ). rewrite inst_trans in Heq.
           exists (inst r12 ι2). split. easy. now exists ι2.
         - intros (ι1 & Heq1 & ι2 & Heq2 & HQ). exists ι2.
@@ -455,12 +570,12 @@ Module Pred.
 
       Lemma wp_false {w0 w1} (r01 : R w0 w1) :
         wp r01 ⊥ₚ ⊣⊢ₚ ⊥ₚ.
-      Proof. firstorder. Qed.
+      Proof. constructor. firstorder. Qed.
 
       Lemma wp_step {stepR : Step R} {w} {x} (Q : Pred (ctx.snoc w x)):
-        wp (w0:=w) step Q ⊣⊢ₚ (∃ₚ t ∶ Ty w, Ext Q (thick (xIn := ctx.in_zero) x t)).
+        wp (w0:=w) step Q ⊣⊢ₚ (∃ₚ t : Ty w, Ext Q (thick (xIn := ctx.in_zero) x t)).
       Proof.
-        intros ι. cbn - [thick]. unfold Exists.
+        constructor. intros ι; pred_unfold; cbn - [thick].
         split.
         - intros (ι' & <- & HQ). destruct (env.view ι') as [ι t].
           rewrite inst_step_snoc. exists (lift t _). cbn - [thick].
@@ -475,7 +590,7 @@ Module Pred.
       Lemma and_wp_l {w0 w1} (r01 : R w0 w1) P Q :
         wp r01 P /\ₚ Q ⊣⊢ₚ wp r01 (P /\ₚ Ext Q r01).
       Proof.
-        split; cbn.
+        constructor. split; cbn.
         - intros [(ι1 & <- & HP) HQ]. now exists ι1.
         - intros (ι1 & <- & HP & HQ). split; [|easy]. now exists ι1.
       Qed.
@@ -484,22 +599,35 @@ Module Pred.
         P /\ₚ wp r01 Q ⊣⊢ₚ wp r01 (Ext P r01 /\ₚ Q).
       Proof. now rewrite and_comm, and_wp_l, and_comm. Qed.
 
+      Lemma wp_reduce {reduceR : Reduce R}
+        {w α} (t : Ty w) (Q : Pred w) :
+        wp (reduce α t) Q ⊣⊢ₚ
+          Ty_hole ctx.in_zero =ₚ (persist _ t _ (step (R := Alloc))) /\ₚ Ext Q (step (R := Alloc)).
+      Proof.
+        constructor. intros ι; pred_unfold; cbn.
+        split.
+        - intros (ι1 & Heq & HQ). subst. now rewrite inst_reduce.
+        - destruct (env.view ι) as [ι t']. cbn. intros [Heq HQ]. subst.
+          exists ι. split; auto. now rewrite inst_reduce.
+      Qed.
+
       Lemma wp_thick {thickR : Thick R} {instThickR : InstThick R}
         {w x} (xIn : ctx.In x w) (t : Ty (ctx.remove xIn)) (Q : Pred (ctx.remove xIn)) :
         wp (thick x t) Q ⊣⊢ₚ Ty_hole xIn =ₚ thin xIn t /\ₚ Ext Q (Sub.thin xIn).
       Proof.
-        intros ι; cbn. rewrite Sub.subst_thin, inst_persist_ty, Sub.inst_thin.
+        constructor. intros ι; pred_unfold; cbn.
+        rewrite Sub.subst_thin, inst_persist, Sub.inst_thin.
         split.
         - intros (ι1 & Heq & HQ). subst.
           now rewrite inst_thick, env.remove_insert, env.lookup_insert.
         - intros [Heq HQ]. exists (env.remove x ι xIn).
-          now rewrite inst_thick, <- Heq, env.insert_remove.
+          rewrite inst_thick. rewrite <- Heq. now rewrite env.insert_remove.
       Qed.
 
       Lemma wlp_refl {reflR : Refl R} {instReflR : InstRefl R}
         {w} (Q : Pred w) : wlp refl Q ⊣⊢ₚ Q.
       Proof.
-        split; cbn.
+        constructor. split; cbn.
         - intros HQ. apply HQ. now rewrite inst_refl.
         - intros HQ ? <-. now rewrite inst_refl in HQ.
       Qed.
@@ -508,7 +636,7 @@ Module Pred.
         {w0 w1 w2} (r01 : R w0 w1) (r12 : R w1 w2) Q :
         wlp (r01 ⊙ r12) Q ⊣⊢ₚ wlp r01 (wlp r12 Q).
       Proof.
-        split; cbn.
+        constructor. split; cbn.
         - intros HQ ι1 Heq1 ι2 Heq2. apply HQ.
           subst. now rewrite inst_trans.
         - intros HQ ι2 Heq. rewrite inst_trans in Heq.
@@ -517,48 +645,59 @@ Module Pred.
 
       Lemma wlp_true {w0 w1} (r01 : R w0 w1) :
         wlp r01 Trueₚ ⊣⊢ₚ Trueₚ.
-      Proof. firstorder. Qed.
+      Proof. constructor. firstorder. Qed.
 
       Lemma wlp_impl {w0 w1} (r01 : R w0 w1) P Q :
         wlp r01 (P ->ₚ Q) ⊢ₚ wlp r01 P ->ₚ wlp r01 Q.
-      Proof. intros ι0. cbn. intros HPQ HP ι1 <-. firstorder. Qed.
+      Proof. constructor. firstorder. Qed.
+
+      Lemma wlp_and {w0 w1} (r01 : R w0 w1) P Q :
+        wlp r01 P /\ₚ wlp r01 Q ⊢ₚ wlp r01 (P /\ₚ Q).
+      Proof. constructor. firstorder. Qed.
 
       Lemma entails_wlp {w0 w1} (r01 : R w0 w1) P Q :
         (Ext P r01 ⊢ₚ Q) <-> (P ⊢ₚ wlp r01 Q).
       Proof.
-        cbv [entails Ext wlp].
-        split.
-        - intros HPQ ι0 HP ι1 <-. revert HP. apply HPQ.
-        - intros HPQ ι1 HP. now apply (HPQ (inst r01 ι1)).
+        split; intros [HPQ]; constructor.
+        - intros ι0 HP ι1 <-. revert HP. apply HPQ.
+        - intros ι1 HP. now apply (HPQ (inst r01 ι1)).
       Qed.
 
       Lemma entails_wp {w0 w1} (r01 : R w0 w1) P Q :
         (P ⊢ₚ Ext Q r01) <-> (wp r01 P ⊢ₚ Q).
       Proof.
-        cbv [entails Ext wp].
-        split.
-        - intros HPQ ι0 (ι1 & <- & HP). now apply HPQ.
-        - intros HPQ ι1 HP. apply (HPQ (inst r01 ι1)).
+        split; intros [HPQ]; constructor.
+        - intros ι0 (ι1 & <- & HP). now apply HPQ.
+        - intros ι1 HP. apply (HPQ (inst r01 ι1)).
           exists ι1. split; auto.
       Qed.
+
+      Lemma wlp_reduce {reduceR : Reduce R} {w α} (t : Ty w) (Q : Pred w) :
+        wlp (reduce α t) Q ⊣⊢ₚ
+          Ty_hole ctx.in_zero =ₚ (persist _ t _ (step (R := Alloc))) ->ₚ Ext Q (step (R := Alloc)).
+      Proof.
+      Admitted.
 
       Lemma wlp_thick {thickR : Thick R} {instThickR : InstThick R}
         {w x} (xIn : ctx.In x w) (t : Ty (ctx.remove xIn)) (Q : Pred (ctx.remove xIn)) :
         wlp (thick x t) Q ⊣⊢ₚ Ty_hole xIn =ₚ thin xIn t ->ₚ Ext Q (Sub.thin xIn).
       Proof.
-        intros ι; cbn. rewrite Sub.subst_thin, inst_persist_ty, Sub.inst_thin.
+        constructor. intros ι; pred_unfold; cbn.
+        rewrite Sub.subst_thin, inst_persist, Sub.inst_thin.
         split; intros HQ.
         - specialize (HQ (env.remove x ι xIn)). intros Heq.
-          rewrite inst_thick, <- Heq, env.insert_remove in HQ. auto.
+          rewrite inst_thick in HQ.
+          rewrite <- Heq in HQ.
+          rewrite env.insert_remove in HQ. auto.
         - intros ι1 Heq. subst.
           rewrite inst_thick, env.remove_insert, env.lookup_insert in HQ.
           now apply HQ.
       Qed.
 
       Lemma wlp_step {stepR : Step R} {w} {x} (Q : Pred (ctx.snoc w x)):
-        wlp (w0:=w) step Q ⊣⊢ₚ (∀ₚ t ∶ Ty w, Ext Q (thick (xIn := ctx.in_zero) x t)).
+        wlp (w0:=w) step Q ⊣⊢ₚ (∀ₚ t : Ty w, Ext Q (thick (xIn := ctx.in_zero) x t)).
       Proof.
-        intros ι. cbn - [thick]. unfold Forall.
+        constructor. intros ι; pred_unfold; cbn - [thick].
         split.
         - intros HQ t. apply HQ.
           rewrite (inst_thick ctx.in_zero t ι). cbn.
@@ -574,106 +713,113 @@ Module Pred.
     End WithAccessibilityRelation.
     (* #[global] Opaque wp. *)
     (* #[global] Opaque wlp. *)
+
   End Acc.
 
-  Lemma pno_cycle {w} (t1 t2 : Ty w) :
-    Ty_subterm t1 t2 ->
-    t1 =ₚ t2  ⊢ₚ  ⊥ₚ.
+  Lemma pno_cycle {w} (t1 t2 : Ty w) (Hsub : Ty_subterm t1 t2) :
+    t1 =ₚ t2 ⊢ₚ ⊥ₚ.
   Proof.
-    intros Hsub ι Heq.
+    constructor. intros ι Heq.
     apply (inst_subterm ι) in Hsub. cbn in Hsub.
     rewrite <- Heq in Hsub. now apply ty_no_cycle in Hsub.
   Qed.
 
+
   (* A predicate-based induction scheme for the typing relation. *)
   Section InductionScheme.
 
-    Context (P : ⊢ Env -> Const expr -> Ty -> Expr -> Pred).
+    Import iris.bi.interface.
+    Import World.notations.
+    Import Pred.notations.
+    Import Pred.proofmode.
+
+    Open Scope pred_scope.
+
+    Context (P : ⊢ʷ Env -> Const expr -> Ty -> Expr -> Pred).
     Context
       {pfalse : forall w,
-          entails (w := w) Trueₚ
-         (∀ₚ G ∶ Env w, ∀ₚ t ∶ Ty w, ∀ₚ e' ∶ Expr w,
-             t =ₚ Ty_bool ->ₚ
-             e' =ₚ (S.pure v_false) ->ₚ
-             P G v_false t e')%P }
-      {ptrue : forall w, entails Trueₚ (w := w)
-         (∀ₚ G ∶ Env w, ∀ₚ t ∶ Ty w, ∀ₚ e' ∶ Expr w,
-             t =ₚ Ty_bool ->ₚ
-             e' =ₚ (S.pure v_true) ->ₚ
-             P G v_true t e')%P }
-      {pif : forall w, entails Trueₚ (w := w)
-         (∀ₚ⁺ G e1 e2 e3 e' e1' e2' e3' t,
-             (G |--ₚ e1; Ty_bool ~> e1') ->ₚ
-             (G |--ₚ e2; t ~> e2') ->ₚ
-             (G |--ₚ e3; t ~> e3') ->ₚ
-             P G e1 Ty_bool e1' ->ₚ
-             P G e2 t e2' ->ₚ
-             P G e3 t e3' ->ₚ
-             e' =ₚ (fun ι0 => e_if (e1' ι0) (e2' ι0) (e3' ι0)) ->ₚ
-             P G (e_if e1 e2 e3) t e')%P }
-      {pvar : forall w (G : Env w) x t e', entails Trueₚ
-         ((resolve x G) =ₚ (Some t) ->ₚ
-          e' =ₚ (fun _ => e_var x) ->ₚ
-          P G (e_var x) t e') }
-      {pabsu : forall w (G : Env w) x t1 t2 t e1 e1' e',
-        entails Trueₚ
-          ((cons (x, t1) G |--ₚ e1; t2 ~> e1') ->ₚ
-           P (cons (x, t1) G) e1 t2 e1' ->ₚ
-           t =ₚ (Ty_func t1 t2) ->ₚ
-           e' =ₚ (fun ι0 => e_abst x (inst t1 ι0) (e1' ι0)) ->ₚ
-           P G (e_absu x e1) t e' )}
-      {pabst : forall w (G : Env w) x t1 t2 e1 e1' e' t,
-          entails Trueₚ
-            ((cons (x, lift t1 w) G |--ₚ e1; t2 ~> e1') ->ₚ
-             P (cons (x, lift t1 w) G) e1 t2 e1' ->ₚ
-             t =ₚ (Ty_func (lift t1 w) t2) ->ₚ
-             e' =ₚ (fun ι0 => e_abst x t1 (e1' ι0)) ->ₚ
-             P G (e_abst x t1 e1) t e')}
-      {papp : forall w (G : Env w) e1 t1 e1' e2 t2 e2' e',
-          entails Trueₚ
-            ((G |--ₚ e1; Ty_func t2 t1 ~> e1') ->ₚ
-             (G |--ₚ e2; t2 ~> e2') ->ₚ
-             P G e1 (Ty_func t2 t1) e1' ->ₚ
-             P G e2 t2 e2' ->ₚ
-             e' =ₚ (fun ι0 => e_app (e1' ι0) (e2' ι0)) ->ₚ
-             P G (e_app e1 e2) t1 e')%P }.
+        ⊢ ∀ G : Env w, ∀ t : Ty w, ∀ e' : Expr w,
+            t =ₚ Ty_bool →
+            e' =ₚ (S.pure v_false) →
+            P G v_false t e' }
+      {ptrue : forall w,
+        ⊢ ∀ G : Env w, ∀ t : Ty w, ∀ e' : Expr w,
+            t =ₚ Ty_bool →
+            e' =ₚ (S.pure v_true) →
+            P G v_true t e' }
+      {pif : forall w,
+        ⊢ ∀ (G : Env w) (e1 e2 e3 : expr) (e' e1' e2' e3' : Expr w) t,
+            (G |--ₚ e1; Ty_bool ~> e1') →
+            (G |--ₚ e2; t ~> e2') →
+            (G |--ₚ e3; t ~> e3') →
+            P G e1 Ty_bool e1' →
+            P G e2 t e2' →
+            P G e3 t e3' →
+            e' =ₚ (fun ι0 => e_if (e1' ι0) (e2' ι0) (e3' ι0)) →
+            P G (e_if e1 e2 e3) t e' }
+      {pvar : forall w,
+        ⊢ ∀ (G : Env w) x t e',
+            resolve x G =ₚ Some t →
+            e' =ₚ (fun _ => e_var x) →
+            P G (e_var x) t e' }
+      {pabsu : forall w,
+        ⊢ ∀ (G : Env w) x t1 t2 t e1 e1' e',
+            (cons (x, t1) G |--ₚ e1; t2 ~> e1') →
+            P (cons (x, t1) G) e1 t2 e1' →
+            t =ₚ (Ty_func t1 t2) →
+            e' =ₚ (fun ι0 => e_abst x (inst t1 ι0) (e1' ι0)) →
+            P G (e_absu x e1) t e' }
+      {pabst : forall w,
+        ⊢ ∀ (G : Env w) x t1 t2 e1 e1' e' t,
+            (cons (x, lift t1 w) G |--ₚ e1; t2 ~> e1') →
+            P (cons (x, lift t1 w) G) e1 t2 e1' →
+            t =ₚ (Ty_func (lift t1 w) t2) →
+            e' =ₚ (fun ι0 => e_abst x t1 (e1' ι0)) →
+            P G (e_abst x t1 e1) t e' }
+      {papp : forall w,
+        ⊢ ∀ (G : Env w) e1 t1 e1' e2 t2 e2' e',
+            (G |--ₚ e1; Ty_func t2 t1 ~> e1') →
+            (G |--ₚ e2; t2 ~> e2') →
+            P G e1 (Ty_func t2 t1) e1' →
+            P G e2 t2 e2' →
+            e' =ₚ (fun ι0 => e_app (e1' ι0) (e2' ι0)) →
+            P G (e_app e1 e2) t1 e' }.
 
     Lemma TPB_ind w G (e : expr) (t : Ty w) (ee : Expr w) :
       (G |--ₚ e; t ~> ee) ⊢ₚ (P G e t ee).
     Proof.
-      intros ι T. hnf in T.
+      constructor. intros ι T. hnf in T.
       remember (inst G ι) as G'.
       remember (inst t ι) as t'.
       remember (inst ee ι) as ee'.
       revert HeqG' Heqt' Heqee'. revert G t ee. revert w ι.
       induction T; cbn; intros; subst.
-      - apply pfalse; cbn; auto.
-      - apply ptrue; cbn; auto.
+      - apply pfalse; cbn; easy.
+      - apply ptrue; cbn; easy.
       - specialize (IHT1 w ι G Ty_bool (fun _ => cnd') eq_refl eq_refl eq_refl).
         specialize (IHT2 w ι G t0      (fun _ => coq') eq_refl eq_refl eq_refl).
         specialize (IHT3 w ι G t0      (fun _ => alt') eq_refl eq_refl eq_refl).
-        eapply pif; cbn; eauto; eauto.
-      - apply pvar; cbn; auto.
+        eapply pif; cbn; eauto; eauto; easy.
+      - apply pvar; cbn; try easy.
         now rewrite resolve_inst in H.
       - specialize (IHT w ι (cons (v, lift vt _) G) (lift t _) (fun _ => e')).
         cbn in IHT. rewrite ?inst_lift in IHT.
         specialize (IHT eq_refl eq_refl eq_refl).
-        eapply pabsu; cbn; eauto; rewrite ?inst_lift; eauto.
+        eapply pabsu; cbn; eauto; rewrite ?inst_lift; try easy.
         change (@inst _ _ (@inst_sem expr) _ ?e ?ι) with (e ι); cbn.
         now rewrite inst_lift.
       - specialize (IHT w ι (cons (v, lift vt _) G) (lift t _) (fun _ => e')).
         cbn in IHT. rewrite ?inst_lift in IHT.
         specialize (IHT eq_refl eq_refl eq_refl).
-        eapply pabst; cbn; eauto; rewrite ?inst_lift; eauto.
+        eapply pabst; cbn; eauto; rewrite ?inst_lift; easy.
       - specialize (IHT1 w ι G (Ty_func (lift t2 _) t) (fun _ => e1')). cbn in IHT1.
         rewrite ?inst_lift in IHT1. specialize (IHT1 eq_refl eq_refl eq_refl).
         specialize (IHT2 w ι G (lift t2 _) (fun _ => e2')).
         rewrite ?inst_lift in IHT2. specialize (IHT2 eq_refl eq_refl eq_refl).
-        eapply papp; cbn; eauto; rewrite ?inst_lift; eauto.
-    Qed.
+        eapply papp; cbn; eauto; rewrite ?inst_lift; easy.
+    Abort.
 
   End InductionScheme.
-
 
 End Pred.
 Export Pred (Pred).
