theories/stlc/Symbolic.v
@@ -1,35 +1,52 @@
 From Coq Require Import
   Classes.Morphisms
   Classes.Morphisms_Prop
-  Lists.List.
+  Lists.List
+  Strings.String.
 
 From Equations Require Import
   Equations.
 
+From iris Require
+  bi.interface
+  proofmode.tactics.
 From Em Require Import
      Definitions Context Environment STLC Prelude Substitution Triangular
      Predicates
-     unification.CorrectnessWithSubstitutions LogicalRelation.
+     LogicalRelation.
 From Em Require
   Unification.
 
 Import ctx.notations.
 Import ListNotations.
 
-Local Notation "<{ A ~ w }>" := (persist _ A _ w).
+#[local] Arguments step : simpl never.
+#[local] Arguments reduce : simpl never.
+#[local] Arguments thick : simpl never.
 
+Lemma lk_step {Θ : ACC} {lkΘ : Lk Θ} {stepΘ : Step Θ} [w α] (αIn : α ∈ w) :
+  lk step αIn = Ty_hole (w ▻ α) α (ctx.in_succ αIn).
+Proof. Admitted.
+
+Lemma lk_refl {Θ : ACC} {lkΘ : Lk Θ} {reflΘ : Step Θ} [w α] (αIn : α ∈ w) :
+  lk refl αIn = Ty_hole w α αIn.
+Proof. Admitted.
+
+#[local] Notation "<{ A ~ w }>" := (persist _ A _ w) (only parsing).
+#[local] Notation "s [ ζ ]" :=
+  (persist _ s _ ζ)
+    (at level 8, left associativity,
+      format "s [ ζ ]").
 
 #[export] Instance persistent_unit {R} : Persistent R Unit :=
   fun w1 u w2 r => u.
 #[export] Instance persistent_prod {R A B} {pRA : Persistent R A} {pRB : Persistent R B} : Persistent R (Prod A B) :=
   fun w1 '(a,b) w2 r => (persist _ a _ r, persist _ b _ r).
+#[export] Instance persistent_option {R A} {pRA : Persistent R A} : Persistent R (Option A) :=
+  fun w1 oa w2 r => option.map (fun a => persist _ a _ r) oa.
 
 Notation Expr := (Sem expr).
 (* TODO: define reader applicative to use ctor of expr to create Expr *)
-
-#[export] Instance Persistent_Sem {R : ACC} {A}
-  {instR : forall w, Inst (R w) (Assignment w)} : Persistent R (Sem A) :=
-  fun w0 a w1 r1 ι1 => a (inst r1 ι1).
 
 #[export] Instance persistpreorder_alloc_ty : PersistPreOrder Alloc Ty.
 Proof.
@@ -73,9 +90,9 @@ Section Generate.
         [ ω₄ ] t_alt <- generate alt <{ Γ ~ ω₁ ⊙ ω₂ ⊙ ω₃ }> ;;
         [ ω₅ ] _     <- assert <{ t_coq ~ ω₄ }>  t_alt ;;
            Ret_Free Ty _ <{ t_coq ~ ω₄ ⊙ ω₅ }>
-    | e_var var =>
-        match (resolve var Γ) with
-        | Some t_var => Ret_Free Ty _ t_var
+    | e_var x =>
+        match (resolve x Γ) with
+        | Some t_x => Ret_Free Ty _ t_x
         | None => Fail_Free Ty Σ
         end
     | e_app f a =>
@@ -104,7 +121,7 @@ Section RunTI.
   (* infer_schematic defines inference without grounding
      of remaining unification variables. *)
   Definition infer_schematic (e : expr) : option (Schematic Ty) :=
-    match Unification.Variant1.solvefree (generate e []%list) with
+    match Unification.Variant1.solvefree (generate e nil) with
     | Some (w; (_, t)) => Some (w; t)
     | None             => None
     end.
@@ -122,72 +139,50 @@ Section TypeReconstruction.
   Import MonadNotations.
   Import World.notations.
 
-  Definition K {A B : Type} : B -> A -> B := fun b a => b.
+  Notation "f <$> a" := (@S.fmap _ _ f _ a) (at level 61, left associativity).
+  Notation "f <*> a" := (@S.app _ _ _ f a) (at level 61, left associativity).
 
-  Definition F1 {A T Z : Type} : (A -> T) -> (Z -> A) -> Z -> T :=
-    fun f a z => f (a z).
+  Definition decode_ty : ⊢ʷ Ty -> Sem ty := fun w t => inst t.
+  #[global] Arguments decode_ty [w] _.
+  Definition decode_env : ⊢ʷ Env -> Sem env := fun w G => inst G.
+  #[global] Arguments decode_env [w] _.
 
-  Definition F2 {A B T Z : Type} : (A -> B -> T) -> (Z -> A) -> (Z -> B) -> Z -> T :=
-    fun f a b z => f (a z) (b z).
-
-  Definition F3 {A B C T Z : Type} : (A -> B -> C -> T) -> (Z -> A) -> (Z -> B) -> (Z -> C) -> Z -> T :=
-    fun f a b c z => f (a z) (b z) (c z).
-
-  Definition decode_Ty : ⊢ Ty -> Sem ty :=
-  fix decode_Ty w t a {struct t} :=
-    match t with
-    | Ty_bool _ => ty_bool
-    | Ty_func _ t1 t2 => ty_func (decode_Ty w t1 a) (decode_Ty w t2 a)
-    | Ty_hole _ x xIn => env.lookup a xIn
-    end.
-
-  Definition decode_Env : ⊢ Env -> Sem env :=
-  fix decode_Env w e a {struct e} :=
+  Fixpoint reconstruct (e : expr) {Σ : World} (Γ : Env Σ) : FreeM (Prod Ty Expr) Σ :=
     match e with
-    | (s, t) :: e' => (s, decode_Ty w t a) :: decode_Env w e' a
-    | nil          => nil
-    end.
-
-
- Fixpoint reconstruct (e : expr) {Σ : World} (Γ : Env Σ) : FreeM (Prod Ty Expr) Σ :=
-    match e with
-    | v_true  => ret (Ty_bool Σ, K v_true)
-    | v_false => ret (Ty_bool Σ, K v_false)
+    | v_true  => ret (Ty_bool Σ, S.pure v_true)
+    | v_false => ret (Ty_bool Σ, S.pure v_false)
     | e_if cnd coq alt =>
-        [ ω1 ] r_cnd <- reconstruct cnd Γ ;;
-        [ ω2 ] _     <- assert (fst r_cnd) (Ty_bool _) ;;
+        [ ω1 ] '(t1,e1') <- reconstruct cnd Γ ;;
+        [ ω2 ] _     <- assert (Ty_bool _) t1 ;;
         [ ω3 ] r_coq <- reconstruct coq <{ Γ ~ ω1 ⊙ ω2 }> ;;
         [ ω4 ] r_alt <- reconstruct alt <{ Γ ~ ω1 ⊙ ω2 ⊙ ω3 }> ;;
         [ ω5 ] _     <- assert <{ (fst r_coq) ~ ω4 }> (fst r_alt) ;;
-           let e_cnd := <{ (snd r_cnd) ~ ω2 ⊙ ω3 ⊙ ω4 ⊙ ω5 }> in
+           let e_cnd := <{ e1' ~ ω2 ⊙ ω3 ⊙ ω4 ⊙ ω5 }> in
            let e_coq := <{ (snd r_coq) ~ ω4 ⊙ ω5 }> in
            let t_coq := <{ (fst r_coq) ~ ω4 ⊙ ω5 }> in
            let e_alt := <{ (snd r_alt) ~ ω5 }> in
-           ret (t_coq, F3 e_if e_cnd e_coq e_alt)
-    | e_var var =>
-        match (resolve var Γ) with
-        | Some t_var => ret (t_var, F1 e_var (K var))
+           ret (t_coq, e_if <$> e_cnd <*> e_coq <*> e_alt)
+    | e_var x =>
+        match (resolve x Γ) with
+        | Some t_x => ret (t_x, S.pure (e_var x))
         | None => fail
         end
-    | e_app f a =>
-        [ ω1 ] T_cod <- exists_Ty Σ ;;
-        [ ω2 ] r_dom <- reconstruct a <{ Γ ~ ω1 }> ;;
-        [ ω3 ] r_fun <- reconstruct f <{ Γ ~ ω1 ⊙ ω2 }> ;;
-        [ ω4 ] _     <- assert (fst r_fun) <{ (Ty_func _ (fst r_dom) <{ T_cod ~ ω2 }> ) ~ ω3 }> ;;
-           let e_fun := <{ (snd r_fun) ~ ω4 }> in
-           let t_cod := <{ T_cod ~ ω2 ⊙ ω3 ⊙ ω4 }> in
-           let e_dom := <{ (snd r_dom) ~ ω3 ⊙ ω4 }> in
-            ret (t_cod , F2 e_app e_fun e_dom)
-    | e_abst var t_var e =>
-        let t_var' := (lift t_var Σ) in (* t_var lives in ty, not in (Ty w) *)
-        [ ω1 ] t_e <- reconstruct e ((var, t_var') :: Γ) ;;
-          ret (Ty_func _ <{ t_var' ~ ω1 }> (fst t_e),
-              F3 e_abst (K var) (K t_var) (snd t_e))
-    | e_absu var e =>
-        [ ω1 ] t_var <- exists_Ty Σ ;;
-        [ ω2 ] t_e <- reconstruct e ((var, t_var) :: <{ Γ ~ ω1 }>) ;;
-          ret (Ty_func _ <{ t_var ~ ω2 }> (fst t_e),
-              F3 e_abst (K var) (inst <{ t_var ~ ω2 }>) (snd t_e))
+    | e_absu x e1 =>
+        [ ω1 ] t1        <- exists_Ty Σ ;;
+        [ ω2 ] '(t2,e1') <- reconstruct e1 ((x, t1) :: Γ[ω1]) ;;
+          ret (Ty_func _ t1[ω2] t2,
+              e_abst x <$> decode_ty t1[ω2] <*> e1')
+    | e_abst x t_x e =>
+        let t_x' := lift t_x Σ in
+        [ ω1 ] t_e <- reconstruct e ((x, t_x') :: Γ) ;;
+          ret (Ty_func _ t_x'[ω1] (fst t_e),
+              e_abst x t_x <$> snd t_e)
+    | e_app e1 e2 =>
+        [ θ1 ] '(tf, e1') <- reconstruct e1 Γ ;;
+        [ θ2 ] '(t1, e2') <- reconstruct e2 (persist _ Γ _ θ1) ;;
+        [ θ3 ] t2         <- @exists_Ty _ ;;
+        [ θ4 ] _          <- assert tf[θ2⊙θ3] (Ty_func _ t1[θ3] t2) ;;
+            ret (t2[θ4] , e_app <$> e1'[θ2⊙θ3⊙θ4] <*> e2'[θ3⊙θ4])
     end.
 
   Import SigTNotations.
@@ -196,7 +191,7 @@ Section TypeReconstruction.
   (* reconstruct_schematic defines type reconstruction without grounding
      of remaining unification variables. *)
   Definition reconstruct_schematic (e : expr) : option (Schematic (Prod Ty Expr)) :=
-    match Unification.Variant1.solvefree (reconstruct e []%list) with
+    match Unification.Variant1.solvefree (reconstruct e nil) with
     | Some (w; (_, te)) => Some (w; te)
     | None              => None
     end.
@@ -308,35 +303,930 @@ End acc.
 
 Section MoveMe.
 
-  Import (hints) Sub.
-  Lemma persist_liftTy : forall (w w' : World) t (r : Sub w w'),
-      persist w (lift t _) w' r = lift t _.
+  Context {Θ : ACC } {persΘ : Persistent Θ Ty}.
+  Lemma persist_liftTy (w w' : World) t (θ : Θ w w') :
+    persist w (lift t _) w' θ = lift t _.
   Proof.
-    intros w w' t. revert w'.
-    induction t; cbn; intros; now f_equal.
-  Qed.
+    (* intros w w' t. revert w'. *)
+    (* induction t; cbn; intros; now f_equal. *)
+  Admitted.
 
   (* Lemma persist_split : forall w w' iw (pos : w ↑ iw) (neg : iw ↓ w') x, *)
   (*   persist w  x iw pos -> *)
   (*   persist iw x w' neg -> *)
   (*   persist w  x w' {| iw := iw; pos := pos; neg := neg |}. *)
 
-  Lemma persist_liftEnv : forall (w w' : World) e (r : Sub w w'),
-      persist w (liftEnv e _) w' r = liftEnv e _.
+  Lemma persist_liftEnv (w w' : World) e (θ : Θ w w') :
+      persist w (liftEnv e _) w' θ = liftEnv e _.
   Proof.
-    induction e. now cbn.
-    destruct a. cbn. intro r. rewrite IHe.
-    now rewrite persist_liftTy.
-  Qed.
-
-  Lemma subst_lift (t : ty) :
-    forall w1 w2 (r : w1 ⊒ˢ w2),
-      persist _ (lift t w1) _ r = lift t w2.
-  Proof.
-    induction t; intros w1 w2 r; cbn; now f_equal.
-  Qed.
+    (* induction e. now cbn. *)
+    (* destruct a. cbn. intro r. rewrite IHe. *)
+    (* now rewrite persist_liftTy. *)
+  Admitted.
 
 End MoveMe.
+
+
+Section WithPredicates.
+
+  Import World.notations.
+  Import Pred Pred.notations.
+  Import (hints) Pred Pred.Acc Sub.
+
+  Definition WP {A} : ⊢ʷ FreeM A -> □⁺(A -> Pred) -> Pred :=
+    fix WP (w : World) (m : FreeM A w) (POST : □⁺(A -> Pred) w) {struct m} :=
+      match m with
+      | Ret_Free _ _ v => POST _ refl v
+      | Fail_Free _ _ => ⊥ₚ
+      | Bind_AssertEq_Free _ _ t1 t2 k => t1 =ₚ t2 /\ₚ WP w k POST
+      | Bind_Exists_Free _ _ α k =>
+          ∃ₚ t : Ty w,
+           Ext (WP (w ▻ α) k (fun w1 r01 => _4 POST step r01)) (reduce (R := Sub) α t)
+      end%P.
+
+  Definition WLP {A} : ⊢ʷ FreeM A -> □⁺(A -> Pred) -> Pred :=
+    fix WLP (w : World) (m : FreeM A w) (POST : □⁺(A -> Pred) w) {struct m} :=
+      match m with
+      | Ret_Free _ _ v => POST _ refl v
+      | Fail_Free _ _ => ⊤ₚ
+      | Bind_AssertEq_Free _ _ t1 t2 k => t1 =ₚ t2 ->ₚ WLP w k POST
+      | Bind_Exists_Free _ _ α k =>
+          (* ∀ₚ t : Ty w, *)
+          (*   Ext (WLP (w ▻ α) k (fun w1 r01 => _4 POST step r01)) (reduce (R := Sub) α t) *)
+          Acc.wlp step (WLP (w ▻ α) k (fun w1 r01 => _4 POST step r01))
+      end%P.
+
+  Lemma wp_bind {A B w1} (m : FreeM A w1) (f : □⁺(A -> FreeM B) w1) :
+    forall (Q : □⁺(B -> Pred) w1),
+      WP w1 (bind m f) Q ⊣⊢ₚ
+      WP w1 m (fun w1 r01 a => WP w1 (f _ r01 a) (_4 Q r01)).
+  Proof. split; intros; induction m; cbn; firstorder; exists x; firstorder. Qed.
+
+  Lemma wlp_bind {A B w1} (m : FreeM A w1) (f : □⁺(A -> FreeM B) w1) :
+    forall (Q : □⁺(B -> Pred) w1),
+      WLP w1 (bind m f) Q ⊣⊢ₚ
+      WLP w1 m (fun w1 r01 a => WLP w1 (f _ r01 a) (_4 Q r01)).
+  Proof. (* split; intros; induction m; cbn; firstorder; exists x; firstorder. *) Admitted.
+
+  Lemma wp_monotonic' {A w} (m : FreeM A w) (R : Pred w) (P Q : □⁺(A -> Pred) w) :
+    (forall w1 (r : Alloc w w1) (a : A w1),
+        Ext R r ⊢ₚ P w1 r a ->ₚ Q w1 r a) ->
+    R ⊢ₚ WP w m P ->ₚ WP w m Q.
+  Proof. Admitted.
+
+  Lemma wlp_monotonic' {A w} (m : FreeM A w) (R : Pred w) (P Q : □⁺(A -> Pred) w) :
+    (forall w1 (r : Alloc w w1) (a : A w1),
+        Ext R r ⊢ₚ P w1 r a ->ₚ Q w1 r a) ->
+    R ⊢ₚ WLP w m P ->ₚ WLP w m Q.
+  Proof.
+    intros pq. destruct m; cbn.
+    - specialize (pq w refl a). rewrite ext_refl in pq. apply pq.
+    - apply impl_and_adjoint. apply true_r.
+    - admit.
+    - apply impl_and_adjoint. admit.
+  Admitted.
+
+  Lemma wp_frame2 {A w} (m : FreeM A w) (P : □⁺(A -> Pred) w) (Q : Pred w) :
+    WP w m P /\ₚ Q ⊣⊢ₚ WP w m (fun _ θ a => P _ θ a /\ₚ Ext Q θ)%P.
+  Proof. Admitted.
+
+  (* Lemma completeness e : forall (w0 : World) (G : Env w0) {t ee}, *)
+  (*   (TPB G e t ee) *)
+  (*   ⊢ₚ *)
+  (*   WP w0 (reconstruct e G) *)
+  (*       (fun w1 r01 '(t', ee') => (<{ ee ~ r01 }> =ₚ ee' /\ₚ <{ t ~ r01 }> =ₚ t')%P). *)
+  (* Proof. *)
+  (*   intros. revert w0 G e t ee. apply TPB_ind; cbn. *)
+  (*   - intro w. *)
+  (*     apply forall_r. intros _. *)
+  (*     apply forall_r. intros t. *)
+  (*     apply forall_r. intros ee ι. *)
+  (*     unfold T. cbn. intros _ Ht Hee. *)
+  (*     now rewrite inst_persist_ty, inst_refl. *)
+  (*   - intro w. *)
+  (*     apply forall_r. intros _. *)
+  (*     apply forall_r. intros t. *)
+  (*     apply forall_r. intros ee ι. *)
+  (*     unfold T. cbn. intros _ Ht Hee. *)
+  (*     now rewrite inst_persist_ty, inst_refl. *)
+  (*   - intro w1. *)
+  (*     do 9 (apply forall_r; intros ?). *)
+  (*     do 7 (rewrite <- impl_and_adjoint). *)
+  (*     assert (MASSAGE: forall w (A B C D E F G : Pred w), *)
+  (* bientails (andₚ (andₚ (andₚ (andₚ (andₚ (andₚ A B) C) D) E) F) G) *)
+  (*           (andₚ (andₚ (andₚ (andₚ (andₚ (andₚ A B) C) G) E) F) D)) by admit. *)
+  (*     rewrite MASSAGE. clear MASSAGE. *)
+  (*     rewrite wp_bind. apply impl_and_adjoint. apply wp_monotonic'. *)
+  (*     intros w2 r12 [t1 ee1]. cbn -[step]. unfold Definitions.T, _4. *)
+  (*     rewrite wp_bind. *)
+  (*     rewrite <- impl_and_adjoint. *)
+  (*     rewrite (eqₚ_sym t1). *)
+  (*     assert (MASSAGE: forall w (A B C D : Pred w), *)
+  (*                entails (andₚ A (andₚ B C)) (andₚ C D) <-> entails (andₚ A (andₚ B ⊤ₚ)) D) by admit. *)
+  (*     rewrite (MASSAGE _ _ (eqₚ (persist w1 x4 w2 r12) ee1) (eqₚ (Ty_bool w2) t1) _). *)
+  (*     rewrite and_true_r. *)
+  (*     admit. *)
+  (*   - intros w G s t e' ι. cbn. *)
+  (*     intros _ Heqo Hvar. destruct (resolve s G) eqn:?; cbn; inversion Heqo. *)
+  (*     unfold T. firstorder. now rewrite refl_persist. *)
+  (*   - admit. *)
+  (*   - admit. *)
+  (*   - admit. *)
+  (* Admitted. *)
+
+  Lemma soundness' e : forall (w0 : World) (G : Env w0),
+    Trueₚ
+    ⊢ₚ
+    WLP w0 (reconstruct e G)
+        (fun w1 r01 '(t, ee) => TPB <{G ~ r01}> e t ee).
+  Proof.
+    (* induction e; cbn; intros; subst; unfold T. *)
+    (* - constructor; constructor. *)
+    (* - constructor; constructor. *)
+    (* - rewrite wlp_bind. rewrite IHe1. *)
+    (*   rewrite <- and_true_l. apply impl_and_adjoint. apply wlp_monotonic'. *)
+    (*   intros. rewrite ext_true. *)
+    (*   destruct a. rewrite <- impl_and_adjoint. *)
+    (*   cbn. rewrite <- impl_and_adjoint. unfold T. rewrite wlp_bind. *)
+    (*   specialize (IHe2 w1 <{ G ~ r ⊙ refl }>). rewrite IHe2. *)
+    (*   (* probably doable with some kind of tactic, perhaps change or replace X with Y is easier? *) *)
+    (*   assert (MASSAGE: forall w (X Y Z : Pred w), bientails (andₚ (andₚ X Y) Z) (andₚ (andₚ Y Z) X)). *)
+    (*   { intros. now rewrite (and_assoc X _), (and_comm _ X). } *)
+    (*   rewrite MASSAGE. clear MASSAGE. *)
+    (*   apply impl_and_adjoint. apply wlp_monotonic'. *)
+    (*   intros. destruct a. rewrite wlp_bind. *)
+    (*   rewrite <- impl_and_adjoint. rewrite <- and_true_r. *)
+    (*   rewrite IHe3. *)
+    (*   apply impl_and_adjoint. apply wlp_monotonic'. *)
+    (*   intros. destruct a. cbn. unfold T, _4. clear. *)
+    (*   rewrite trans_refl_r, trans_refl_r. *)
+    (*   constructor. *)
+    (*   intro. unfold Ext. unfold andₚ, implₚ, TPB. intros. *)
+    (*   destruct H as [[]]. *)
+    (*   constructor. *)
+    (*   + rewrite inst_persist_env, ?inst_trans. *)
+    (*     rewrite inst_persist_env, H2 in H. cbn in H. *)
+    (*     rewrite persist_trans. *)
+    (*     exact H. *)
+    (*   + rewrite inst_persist_env, inst_trans, inst_trans, inst_persist_ty. *)
+    (*     rewrite inst_persist_env, inst_persist_env in H3. *)
+    (*     apply H3. *)
+    (*   + rewrite inst_persist_env, inst_trans, inst_trans. *)
+    (*     rewrite inst_persist_env, inst_persist_env, inst_trans, <- H1 in H0. *)
+    (*     apply H0. *)
+    (* - destruct (resolve s G) eqn:?; cbn; try easy. *)
+    (*   unfold T. rewrite refl_persist. constructor. constructor. *)
+    (*   now rewrite resolve_inst, Heqo. *)
+    (* - rewrite <- Acc.entails_wlp. rewrite ext_true. rewrite IHe. *)
+    (*   rewrite <- and_true_l. *)
+    (*   apply impl_and_adjoint. unfold T, _4. rewrite wlp_bind. *)
+    (*   apply wlp_monotonic'. *)
+    (*   intros. rewrite ext_true. *)
+    (*   destruct a. cbn -[step]. unfold T, _4. *)
+    (*   rewrite trans_refl_r, trans_refl_r. *)
+    (*   constructor. intro. cbn -[step]. *)
+    (*   unfold Ext, andₚ, implₚ, TPB. intros. cbn -[step] in *. *)
+    (*   constructor. rewrite ?inst_persist_env in *. exact H0. *)
+    (* - rewrite wlp_bind. specialize (IHe w0 ((s, lift t w0) :: G)). rewrite IHe. *)
+    (*   rewrite <- and_true_l. *)
+    (*   apply impl_and_adjoint. *)
+    (*   apply wlp_monotonic'. *)
+    (*   intros. rewrite ext_true. destruct a. rewrite <- impl_and_adjoint. *)
+    (*   rewrite and_true_l. cbn in *. unfold T, _4. *)
+    (*   constructor. intros ι He. cbn in *. rewrite ?inst_persist_env, ?inst_persist_ty, ?trans_refl_r, ?inst_lift in *. now constructor. *)
+    (* - rewrite <- Acc.entails_wlp, ext_true, IHe2, <- and_true_l. *)
+    (*   apply impl_and_adjoint. unfold T, _4. rewrite wlp_bind. apply wlp_monotonic'. *)
+    (*   intros w1 r [t2 e2']. *)
+    (*   rewrite ext_true, wlp_bind, <- impl_and_adjoint, and_comm, IHe1. *)
+    (*   apply impl_and_adjoint. apply wlp_monotonic'. *)
+    (*   intros w2 r12 [t1 e1']. cbn -[step]. unfold T, _4. *)
+    (*   rewrite ?trans_refl_r. *)
+    (*   constructor. *)
+    (*   intros ι He2 He1 Ht1. *)
+    (*   cbn -[step] in *. *)
+    (*   rewrite ?inst_persist_ty, ?inst_persist_env, ?inst_trans, ?assoc_persist in *. *)
+    (*   rewrite Ht1 in He1. econstructor. *)
+    (*   exact He1. exact He2. *)
+  Admitted.
+
+  Import bi.interface.
+  Import Pred.proofmode.
+  #[local] Open Scope pred_scope.
+
+
+  Lemma wlp_mono (A : TYPE) (w : World) (m : FreeM A w) (P Q : □⁺(A -> Pred) w) :
+    (∀ (w1 : World) (r : Alloc w w1) (a : A w1), Acc.wlp r (P w1 r a → Q w1 r a)) ⊢
+    (WLP w m P -∗ WLP w m Q).
+  Proof. Admitted.
+
+  Lemma wp_mono (A : TYPE) (w : World) (m : FreeM A w) (P Q : □⁺(A -> Pred) w) :
+    (∀ (w1 : World) (r : Alloc w w1) (a : A w1), Acc.wlp r (P w1 r a → Q w1 r a)) ⊢
+    (WP w m P -∗ WP w m Q).
+  Proof. Admitted.
+
+
+End WithPredicates.
+
+Module ProgramLogic.
+
+  Export Pred (* Pred.notations *).
+  Export (hints) Pred.Acc.
+  Export (hints) alloc.
+  Export (hints) Sub.
+  Export Pred.notations.
+
+  Lemma ext_wp_step {w0 w1 : World} (x : nat) (P : Pred (w0 ▻ x)) (θ : Sub w0 w1) :
+    Ext (Acc.wp (step (R := Alloc)) P) θ ⊣⊢ₚ
+      Acc.wp (step (R := Alloc)) (Ext P (Sub.up1 θ)).
+  Proof.
+    rewrite !Acc.wp_step. constructor.
+    intros ι; cbn - [thick Sub.up1].
+    split; intros [t HP].
+    - exists (persist _ t _ θ). admit.
+    - exists (lift (inst t ι) _). admit.
+  Admitted.
+
+  Lemma step_reduce {Θ1 Θ2 T} `{Persistent Θ1 T, Persistent Θ2 T, Step Θ1, Reduce Θ2} {w α s} (t : T w) :
+    persist _ (persist w t (w ▻ α) (step (R := Θ1))) _ (reduce (R := Θ2) α s) = t.
+  Proof. Admitted.
+
+  Lemma lift_reduce {Θ} `{Persistent Θ Ty, Reduce Θ} w α s t :
+    (lift t (w ▻ α))[reduce (R := Θ) α s] = lift t w.
+  Proof. Admitted.
+
+  Lemma eqₚ_env_cons {w} b1 b2 (G1 G2 : Env w) :
+    cons b1 G1 =ₚ cons b2 G2 ⊣⊢ₚ
+    b1 =ₚ b2 /\ₚ G1 =ₚ G2.
+  Proof.
+    destruct b1, b2. constructor. intros ι. pred_unfold. cbn. split.
+    - injection 1. intuition.
+    - intros []. f_equal; auto.
+  Qed.
+
+  Lemma eq_func {w} (s1 s2 t1 t2 : Ty w) :
+    Ty_func w s1 s2 =ₚ Ty_func w t1 t2 ⊣⊢ₚ (s1 =ₚ t1) /\ₚ (s2 =ₚ t2).
+  Proof. now rewrite peq_ty_noconfusion. Qed.
+
+  Import bi.interface.
+  Import Pred.proofmode.
+  #[local] Open Scope pred_scope.
+
+  Definition ext_gen {w0} (P : Pred w0) {w1} (r01 : Sub w0 w1) (HP : ⊢ P) : ⊢ Ext P r01 :=
+    {| fromEntails ι _ := fromEntails HP (inst r01 ι) (MkEmp (inst r01 ι)) |}.
+  #[global] Arguments ext_gen {w0 P w1} r01 HP.
+
+  Lemma ext_impl' (Θ : ACC) (instΘ : forall w, Inst (Θ w) (Assignment w)) {w0 w1}
+    (θ01 : Θ w0 w1) (P Q : Pred w0) :
+    Ext (P → Q) θ01 ⊣⊢ (Ext P θ01 → Ext Q θ01).
+  Proof. apply ext_impl. Qed.
+
+  Lemma equiv_true {w} : @Trueₚ w ⊣⊢ True.
+  Proof. easy. Qed.
+
+  Lemma equiv_sep {w} (P Q : Pred w) : (P ∗ Q) ⊣⊢ (P ∧ Q).
+  Proof. constructor. firstorder. Qed.
+
+  Lemma equiv_wand {w} (P Q : Pred w) : (P -∗ Q) ⊣⊢ (P → Q).
+  Proof. constructor. firstorder. Qed.
+
+  Lemma resolve_eq {w} {G1 G2 : Env w} x :
+    G1 =ₚ G2 ⊢ₚ resolve x G1 =ₚ resolve x G2.
+  Proof. constructor. intros ι ?. cbn. rewrite <- !resolve_inst. now f_equal. Qed.
+
+  Lemma resolve_persist {R : ACC} `{Definitions.Persistent R Ty}
+    {w0 w1} (r01 : R w0 w1) (G : Env w0) (x : string) :
+    resolve x G[r01] = (resolve x G)[r01].
+  Proof. induction G as [|[y]]; cbn; [|destruct string_dec]; easy. Qed.
+
+  Lemma eqₚ_trans'
+    {w} : ⊢ ∀ (s t u : Option Ty w), s =ₚ t → t =ₚ u → s =ₚ u.
+  Proof.
+    constructor. intros ι _ s t u st tu.
+    exact (fromEntails (eqₚ_trans _ _ _) ι (conj st tu)).
+  Qed.
+
+  Lemma lk_reduce_zero {w x} (t : Ty w) :
+    lk (reduce (R := Sub) x t) ctx.in_zero = t.
+  Proof. reflexivity. Qed.
+
+  Lemma lk_reduce_succ {w x y} (t : Ty w) (yIn : y ∈ w) :
+    lk (reduce (R := Sub) x t) (ctx.in_succ yIn) = Ty_hole w y yIn.
+  Proof. exact (env.lookup_tabulate (Ty_hole w) yIn). Qed.
+
+  Lemma ext_wlp {R} {instR : forall w, Inst (R w) (Assignment w)}
+    {w0 w1} {r01 : R w0 w1} P :
+    Ext (Acc.wlp r01 P) r01 ⊢ₚ P.
+  Proof. constructor. intros ι H. now apply H. Qed.
+
+  Lemma lookup_inst {w1 w2 : World} (r : Alloc w1 w2) (ι : Assignment w2) {x} (i : x ∈ w1) :
+    env.lookup (inst r ι) i = env.lookup ι i[r].
+  Proof. induction r. reflexivity. cbn. rewrite <- IHr. now destruct env.view. Qed.
+
+End ProgramLogic.
+
+Ltac wsimpl :=
+  repeat
+    (rewrite ?persist_refl, ?persist_trans, ?persist_liftEnv, ?persist_liftTy,
+      ?inst_lift, ?inst_reduce, ?inst_persist,
+      ?inst_step_snoc, ?inst_lift_env, ?Sub.lk_trans, ?trans_refl_l, ?trans_refl_r,
+
+      ?Pred.ext_refl, ?Pred.ext_tpb, ?Pred.ext_and, ?Pred.ext_eq,
+      ?Pred.eqₚ_refl, ?Pred.impl_true_l, ?Pred.and_true_r, ?Pred.and_true_l,
+      ?Pred.impl_true_r, ?Pred.impl_false_l, ?Pred.ext_impl, ?Pred.impl_and,
+      ?Pred.ext_exists, ?Pred.ext_forall, ?Pred.Acc.wlp_true, ?Pred.eq_pair,
+
+      ?Sub.persist_sim_step_alloc_env, ?Sub.persist_sim_step_alloc_ty, ?Sub.persist_sim_step_alloc_sem,
+
+      ?ProgramLogic.eqₚ_env_cons, ?ProgramLogic.step_reduce,
+      ?ProgramLogic.lift_reduce, ?ProgramLogic.eq_func,
+      ?ProgramLogic.equiv_true, ?ProgramLogic.lk_reduce_zero,
+      ?ProgramLogic.lk_reduce_succ;
+     cbn - [lk trans step thin thick Sub.up1]; auto);
+  repeat setoid_rewrite Pred.ext_exists;
+  repeat setoid_rewrite Pred.ext_forall;
+  repeat
+    match goal with
+    | |- context[@persist ?Θ ?A ?I ?w0 ?x ?w1 ?r01] =>
+        is_var x; generalize (@persist Θ A I w0 x w1 r01); clear x; intros x;
+        try (clear w0 r01)
+    | |- context[fun w : Ctx nat => Ty w] =>
+        change_no_check (fun w : Ctx nat => Ty w) with Ty
+    | |- context[fun w : Ctx nat => Sem ?X w] =>
+        change_no_check (fun w : Ctx nat => Sem X w) with (Sem X)
+    end.
+
+Section Modalities.
+
+  Import Pred Pred.notations.
+  Import (hints) Sub.
+  Import ProgramLogic Pred.proofmode.
+  Import iris.proofmode.tactics.
+  Open Scope pred_scope.
+
+  Section AccModality.
+
+    Context {Θ : ACC} (instΘ : forall w, Inst (Θ w) (Assignment w)) [w0 w1] (θ : Θ w0 w1).
+
+    Class IntoAcc (P : Pred w0) (Q : Pred w1) :=
+      into_acc : P ⊢ Acc.wlp θ Q.
+
+    #[export] Instance into_acc_default (P : Pred w0) : IntoAcc P (Ext P θ).
+    Proof. constructor. cbn. intros ι0 HP ι1 <-. apply HP. Qed.
+
+    Definition modality_wlp_mixin :
+      modality_mixin (Acc.wlp θ)
+        (MIEnvTransform IntoAcc)
+        (MIEnvTransform IntoAcc).
+    Proof. firstorder. Qed.
+
+    Definition modality_wlp : modality bi_pred bi_pred :=
+      Modality _ (modality_wlp_mixin).
+
+    #[export] Instance from_modal_wlp P :
+      FromModal True modality_wlp (Acc.wlp θ P) (Acc.wlp θ P) P.
+    Proof. firstorder. Qed.
+
+  End AccModality.
+
+  #[global] Arguments IntoAcc {Θ _} [w0 w1] θ P Q.
+  #[global] Arguments into_acc {Θ _} [w0 w1] θ P Q {_}.
+  #[global] Hint Mode IntoAcc + + + + + - - : typeclass_instances.
+
+  Section ExtReduceModality.
+
+    Context {Θ : ACC} (instΘ : forall w, Inst (Θ w) (Assignment w)).
+    Context [w : World] (α : nat) (t : Ty w).
+
+    Class IntoExtReduce (P : Pred w) (Q : Pred (w ▻ α)) :=
+      into_ext_reduce : P ⊢ Ext Q (reduce α t).
+
+    #[export] Instance into_ext_reduce_default (P : Pred w) :
+      IntoExtReduce P (Ext P (step (R := Sub))).
+    Proof.
+      constructor. cbn - [inst step]. intros ι HP.
+      now rewrite inst_reduce inst_step_snoc.
+    Qed.
+
+    Definition modality_ext_reduce_mixin :
+      modality_mixin (fun P => Ext P (reduce α t))
+        (MIEnvTransform IntoExtReduce)
+        (MIEnvTransform IntoExtReduce).
+    Proof. firstorder. Qed.
+
+    Definition modality_ext_reduce : modality bi_pred bi_pred :=
+      Modality _ (modality_ext_reduce_mixin).
+
+    #[export] Instance from_modal_ext_reduce P :
+      FromModal True modality_ext_reduce
+        (Ext P (reduce α t)) (Ext P (reduce α t))
+        (persist w t (ctx.snoc w α) (step (R := Sub)) =ₚ Ty_hole (w ▻ α) α ctx.in_zero ->ₚ P).
+    Proof.
+      intros _. cbn. apply ext_reduce. constructor. pred_unfold.
+      intros ι. cbn. destruct (env.view ι) as [ι t'].
+      rewrite ?inst_persist ?inst_reduce inst_step_snoc. cbn.
+      rewrite inst_step_snoc. intros HP ->. now apply HP.
+    Qed.
+
+  End ExtReduceModality.
+
+End Modalities.
+
+(* Focus on the constraint generation only, forget about solving constraints
+   and any semantic values. Also try to pass the type as an input instead of
+   an output, i.e. checking instead of synthesizing. *)
+Module ConstraintsOnly.
+
+  Import option.notations.
+  Import Unification.
+
+  #[local] Set Implicit Arguments.
+
+  Module C.
+
+    Import World.notations.
+    Import Pred Pred.notations.
+    Import (hints) Sub.
+
+    Inductive CStr (w : World) : Type :=
+    | False
+    | Eq (t1 t2 : Ty w)
+    | And (C1 C2 : CStr w)
+    | Ex {x} (C : CStr (w ▻ x)).
+    #[global] Arguments False {w}.
+    #[global] Arguments Ex [w] x C.
+
+    Definition denote : ⊢ʷ CStr -> Pred :=
+      fix den {w} C {struct C} : Pred w :=
+        match C with
+        | False     => ⊥ₚ
+        | Eq t1 t2  => t1 =ₚ t2
+        | And C1 C2 => den C1 /\ₚ den C2
+        | Ex x C    => ∃ₚ t : Ty w, Ext (den C) (reduce (R := Sub) x t)
+        (* | Ex x C    => ∃ₚ t : ty, Ext (den C) (reduce (R := Sub) x (lift t _)) *)
+        (* | Ex x C    => Acc.wlp (step (R := Sub)) (den C) *)
+        end%P.
+
+    Notation "C1 /\ C2" := (C.And C1 C2).
+    Notation "t1 == t2" := (C.Eq t1 t2) (at level 80).
+    Notation "∃ n , C" := (C.Ex n C) (at level 80, right associativity, format "∃ n ,  C").
+  End C.
+  Export C (CStr).
+
+  Section Check.
+    Import World.notations.
+    Import C.
+
+    Fixpoint check (e : expr) : ⊢ʷ Env -> Ty -> CStr :=
+      fun (w : World) (G : Env w) (tr : Ty w) =>
+        match e with
+        | v_true => Ty_bool w == tr
+        | v_false => Ty_bool w == tr
+        | e_if e1 e2 e3 =>
+            check e1 G (Ty_bool w) /\
+            check e2 G tr /\
+            check e3 G tr
+        | e_var s =>
+            match resolve s G with
+            | Some a => tr == a
+            | None => C.False
+            end
+        | e_absu x e =>
+            ∃1, ∃2,
+              let G'  := <{ G ~ step (R := Alloc) ⊙ step }> in
+              let tr' := <{ tr ~ step (R := Alloc) ⊙ step }> in
+              let α1  := Ty_hole (w ▻ 1 ▻ 2) 1 (ctx.in_succ ctx.in_zero) in
+              let α2  := Ty_hole (w ▻ 1 ▻ 2) 2 ctx.in_zero in
+              (Ty_func _ α1 α2 == tr') /\
+              check e ((x, α1) :: G') α2
+        | e_abst x xt e =>
+            ∃2,
+              let G'  := <{ G ~ step (R := Alloc) }> in
+              let tr' := <{ tr ~ step (R := Alloc) }> in
+              let α1  := lift xt _ in
+              let α2  := Ty_hole (w ▻ 2) 2 ctx.in_zero in
+              (Ty_func _ α1 α2 == tr') /\
+              check e ((x, α1) :: G') α2
+        | e_app e1 e2 =>
+            ∃0,
+              let G'  := <{ G ~ step (R := Alloc) }> in
+              let tr' := <{ tr ~ step (R := Alloc) }> in
+              let α   := Ty_hole (w ▻ 0) 0 ctx.in_zero in
+              check e1 G' (Ty_func _ α tr') /\
+              check e2 G' α
+        end.
+
+  End Check.
+
+  Import iris.bi.interface.
+  Import iris.proofmode.tactics.
+  Import Pred Pred.notations Pred.proofmode.
+  Import (hints) Sub.
+
+  Lemma soundness e :
+    forall (w : World) G t,
+      C.denote (check e G t) ⊢ (∃ₚ ee : Expr w, G |--ₚ e; t ~> ee)%P.
+  Proof.
+    induction e; cbn; intros w G tr; wsimpl.
+    - apply exists_r. exists (S.pure v_true).
+      constructor. intros ι. cbn. intros <-. constructor.
+    - apply exists_r. exists (S.pure v_false).
+      constructor. intros ι. cbn. intros <-. constructor.
+    - rewrite IHe1 IHe2 IHe3.
+      iIntros "([%e1' H1] & [%e2' H2] & [%e3' H3])".
+      iExists (fun ι => e_if (e1' ι) (e2' ι) (e3' ι)).
+      iStopProof. constructor. intros ι (IH1 & IH2 & IH3). now constructor.
+    - destruct resolve eqn:?; cbn.
+      + apply exists_r. exists (S.pure (e_var s)).
+        constructor. intros ι. cbn.
+        constructor. now rewrite resolve_inst Heqo H.
+      + apply false_l.
+    - iIntros "(%t1 & %t2 & H)". wsimpl. rewrite IHe. wsimpl.
+      iDestruct "H" as "[Heq [%e' H]]". wsimpl.
+      iExists (fun ι => e_abst s (inst t1 ι) (inst e' ι)).
+      iStopProof. constructor. intros ι (Heq & IH). cbn in *.
+      rewrite <- Heq. now constructor.
+    - iIntros "(%t2 & H)". wsimpl. rewrite IHe. wsimpl.
+      iDestruct "H" as "[Heq [%e' H]]". wsimpl.
+      iExists (fun ι => e_abst s t (inst e' ι)).
+      iStopProof. constructor. intros ι (Heq & IH). cbn in *.
+      rewrite inst_lift in Heq IH. rewrite <- Heq. now constructor.
+    - iIntros "(%t2 & H)". wsimpl. rewrite IHe1 IHe2. wsimpl.
+      iDestruct "H" as "([%e1' H1] & [%e2' H2])". wsimpl.
+      iExists (fun ι => e_app (e1' ι) (e2' ι)).
+      iStopProof. constructor. intros ι (H1 & H2). cbn in *.
+      econstructor; eauto.
+  Qed.
+
+  Import iris.proofmode.tactics.
+  Import ProgramLogic Pred.proofmode.
+  Open Scope pred_scope.
+
+  Lemma completeness_aux {G e t ee} (T : G |-- e; t ~> ee) :
+    forall w0 (G0 : Env w0) (t0 : Ty w0),
+      ⊢ liftEnv G _ =ₚ G0 → lift t _ =ₚ t0 → C.denote (check e G0 t0).
+  Proof.
+    induction T; intros w0 G0 t0; wsimpl.
+    - iIntros "#HeqG #Heqt". repeat iSplit.
+      + iApply IHT1; wsimpl.
+      + iApply IHT2; wsimpl.
+      + iApply IHT3; wsimpl.
+    - constructor. intros ι. intros _ HeqG Heqt. cbn in *.
+      rewrite inst_lift_env in HeqG.
+      rewrite inst_lift in Heqt. subst.
+      rewrite resolve_inst in H.
+      destruct resolve.
+      + injection H. easy.
+      + discriminate H.
+    - iIntros "#HeqG #Heqt".
+      iExists (lift vt w0), (lift t _). wsimpl. iSplit; wsimpl.
+      iIntros "!> #Heq1 !> #Heq2". iApply IHT; wsimpl.
+    - iIntros "#HeqG #Heqt".
+      iExists (lift t _). wsimpl. iSplit; wsimpl.
+      iIntros "!> #Heq1". iApply IHT; wsimpl.
+    - iIntros "#HeqG #Heqt".
+      iExists (lift t2 _). iIntros "!> #Heq1".
+      iSplit.
+      + iApply IHT1; wsimpl.
+      + iApply IHT2; wsimpl.
+  Qed.
+
+  Corollary completeness G e t ee (T : G |-- e ; t ~> ee) :
+    C.denote (check e (liftEnv G _) (lift t _)) env.nil.
+  Proof. eapply completeness_aux; now eauto. Qed.
+
+End ConstraintsOnly.
+
+Module CandidateType.
+
+  Import World.notations.
+
+  #[local] Set Implicit Arguments.
+  #[local] Arguments step : simpl never.
+
+  Section Check.
+    Import World.notations.
+
+    #[local] Notation "[ ω ] x <- ma ;; mb" :=
+      (bind (R := Alloc) ma (fun _ ω x => mb))
+        (at level 80, x at next level,
+          ma at next level, mb at level 200,
+          right associativity).
+
+    #[local] Notation "∃ n , m" :=
+      (Bind_Exists_Free _ _ n m)
+        (at level 80, right associativity, format "∃ n ,  m").
+
+    #[local] Notation "t1 == t2 //\ m" := (Bind_AssertEq_Free _ _ t1 t2 m) (at level 70).
+
+    Fixpoint check (e : expr) : ⊢ʷ Env -> Ty -> FreeM Unit :=
+      fun w G tr =>
+        match e with
+        | v_true => Bind_AssertEq_Free Unit w (Ty_bool w) tr (Ret_Free Unit w tt)
+        | v_false => Bind_AssertEq_Free Unit w (Ty_bool w) tr (Ret_Free Unit w tt)
+        | e_if e0 e1 e2 =>
+          [r1] _ <- check e0 G (Ty_bool w)   ;;
+          [r2] _ <- check e1 G[r1] tr[r1] ;;
+          check e2 G[r1 ⊙ r2] tr[r1 ⊙ r2]
+        | e_var s =>
+          match resolve s G with
+          | Some a => Bind_AssertEq_Free Unit w tr a (Ret_Free Unit w tt)
+          | None => Fail_Free Unit w
+          end
+        | e_absu s e0 =>
+          ∃1, ∃2,
+            let tr' := tr[step ⊙ step] in
+            let α1  := Ty_hole _ 1 (ctx.in_succ ctx.in_zero) in
+            let α2  := Ty_hole _ 2 ctx.in_zero in
+            Ty_func _ α1 α2 == tr' //\
+            check e0 ((s, α1) :: G[step ⊙ step]) α2
+
+        | e_abst s t e0 =>
+          ∃2,
+            let tr' := <{ tr ~ step }> in
+            let α1  := lift t (w ▻ 2) in
+            let α2  := Ty_hole (w ▻ 2) 2 ctx.in_zero in
+            Ty_func (w ▻ 2) α1 α2 == tr' //\
+            check e0 ((s, α1) :: <{ G ~ step }>) α2
+        | e_app e0 e1 =>
+          ∃0,
+            let α := Ty_hole (w ▻ 0) 0 ctx.in_zero in
+            [r1] _ <- check e0 <{ G ~ step }> (Ty_func _ α <{ tr ~ step }>) ;;
+                      check e1 G[step ⊙ r1] <{ α ~ r1 }>
+    end.
+
+  End Check.
+
+  Import Pred Pred.notations.
+  Import (hints) Sub.
+  Import ProgramLogic Pred.proofmode.
+  Import iris.proofmode.tactics.
+  Open Scope pred_scope.
+
+  Lemma soundness (e : expr) :
+    forall (w : World) (G : Env w) (tr : Ty w),
+      ⊢ WLP _ (check e G tr) (fun w1 r1 _ => ∃ₚ ee : Expr w1, G[r1] |--ₚ e; tr[r1] ~> ee).
+  Proof.
+    induction e; cbn; intros w G tr; unfold T, _4; wsimpl.
+    - constructor. intros ι. pred_unfold.
+      exists (S.pure v_true). constructor.
+    - constructor. intros ι. pred_unfold.
+      exists (S.pure v_false). constructor.
+    - rewrite wlp_bind. unfold _4.
+      iPoseProof (IHe1 w G (Ty_bool w)) as "-#IH1". iRevert "IH1". clear IHe1.
+      iApply wlp_mono. iIntros (w1 r1 _). iIntros "!> [%e1' HT1]".
+
+      rewrite wlp_bind. unfold _4.
+      iPoseProof (IHe2 w1 G[r1] tr[r1]) as "-#IH2". iRevert "IH2". clear IHe2.
+      iApply wlp_mono. iIntros (w2 r2 _). iIntros "!> [%e2' HT2]".
+
+      iPoseProof (IHe3 w2 G[r1 ⊙ r2] tr[r1 ⊙ r2]) as "-#IH3". iRevert "IH3". clear IHe3.
+      iApply wlp_mono. iIntros (w3 r3 _). iIntros "!> [%e3' HT3]".
+      wsimpl.
+
+      iExists (fun ι => e_if (e1' ι) (e2' ι) (e3' ι)).
+      iStopProof. constructor. intros ι (IH1 & IH2 & IH3). now constructor.
+    - destruct resolve eqn:?; wsimpl.
+      constructor. intros ι; pred_unfold.
+      exists (S.pure (e_var s)).
+      constructor. now rewrite resolve_inst Heqo.
+    - iIntros "!> !> Heq1".
+      iPoseProof (IHe (w ▻ 1 ▻ 2)
+                      ((s, Ty_hole (w ▻ 1 ▻ 2) 1 (ctx.in_succ ctx.in_zero)) :: G[step][step])
+                      (Ty_hole (w ▻ 1 ▻ 2) 2 ctx.in_zero)) as "-#IH". iRevert "IH". clear IHe.
+      iApply wlp_mono. iIntros (w1 r1 _).
+      iIntros "!> [%e' HT]". wsimpl.
+      iExists (fun ι => e_abst s (inst (lk r1 (ctx.in_succ ctx.in_zero)) ι) (e' ι)).
+      iStopProof. constructor. intros ι (Heq & IH). pred_unfold. now constructor.
+    - iIntros "!> Heq".
+      iPoseProof (IHe (w ▻ 2)
+                    ((s, lift t (w ▻ 2)) :: G[step])
+                    (Ty_hole (w ▻ 2) 2 ctx.in_zero))
+                      as "-#IH". iRevert "IH". clear IHe.
+      iApply wlp_mono. iIntros (w1 r1 _).
+      iIntros "!> [%e' HT]". wsimpl.
+      generalize (lk r1 ctx.in_zero). clear w r1. intros t2.
+      iExists (fun ι => e_abst s t (e' ι)).
+      iStopProof. constructor. intros ι (Heq & IH). pred_unfold. now constructor.
+    - iIntros "!>".
+
+      rewrite wlp_bind. unfold _4.
+      iPoseProof (IHe1 (w ▻ 0) G[step] (Ty_func (w ▻ 0) (Ty_hole (w ▻ 0) 0 ctx.in_zero) tr[step]))
+        as "-#IH". iRevert "IH". clear IHe1.
+      iApply wlp_mono. iIntros (w1 r1 _). iIntros "!> [%e1' HT1]".
+
+      iPoseProof (IHe2 w1 G[step ⊙ r1] (lk r1 ctx.in_zero)) as "-#IH". iRevert "IH". clear IHe2.
+      iApply wlp_mono. iIntros (w2 r2 _). iIntros "!> [%e2' HT2]". wsimpl.
+      generalize (lk r1 ctx.in_zero)[r2]. clear w r1. intros t1.
+      iExists (fun ι => e_app (e1' ι) (e2' ι)).
+      iStopProof. constructor. intros ι (H1 & H2). pred_unfold.
+      econstructor; eauto.
+  Qed.
+
+  Lemma completeness_aux {G e t ee} (T : G |-- e; t ~> ee) :
+    forall w0 (G0 : Env w0) (t0 : Ty w0),
+      ⊢ liftEnv G _ =ₚ G0 → lift t _ =ₚ t0 → WP _ (check e G0 t0) (fun _ _ _ => Trueₚ)%P.
+  Proof.
+    induction T; intros w0 G0 t0; wsimpl.
+    - iIntros "#HeqG #Heqt". rewrite wp_bind.
+      iPoseProof (IHT1 w0 G0 (Ty_bool w0) with "HeqG") as "-#IHT1".
+      clear IHT1. wsimpl.
+      iRevert "IHT1". iApply wp_mono. iIntros (w1 r1 _). wsimpl.
+      iModIntro. wsimpl. rewrite wp_bind.
+      iPoseProof (IHT2 w1 G0[r1] t0[r1] with "HeqG Heqt") as "-#IHT2".
+      iRevert "IHT2". iApply wp_mono. iIntros (w2 r2 _). wsimpl.
+      iModIntro. wsimpl. unfold _4.
+      iApply IHT3; wsimpl.
+    - constructor. intros ι. intros _ HeqG Heqt. cbn in *.
+      rewrite inst_lift_env in HeqG.
+      rewrite inst_lift in Heqt. subst.
+      rewrite resolve_inst in H.
+      destruct resolve.
+      + injection H. easy.
+      + discriminate H.
+    - iIntros "#HeqG #Heqt".
+      iExists (lift vt _), (lift t _). wsimpl.
+      iSplit. wsimpl.
+      iModIntro. iIntros "#Heq1". iModIntro. iIntros "#Heq2".
+      iPoseProof (IHT (w0 ▻ 1 ▻ 2)
+                    ((v, Ty_hole (w0 ▻ 1 ▻ 2) 1 (ctx.in_succ ctx.in_zero)) :: G0[step][step])
+                    (Ty_hole (w0 ▻ 1 ▻ 2) 2 ctx.in_zero)) as "IHT". clear IHT.
+      wsimpl.
+      iPoseProof ("IHT" with "Heq1 HeqG Heq2") as "-#IHT'". iRevert "IHT'". iClear "IHT".
+      iApply wp_mono. unfold _4. iIntros (w1 r1 _). wsimpl.
+    - iIntros "#HeqG #Heqt".
+      iExists (lift t _). wsimpl.
+      iSplit. wsimpl.
+      iModIntro. iIntros "#Heq1".
+      iPoseProof (IHT (w0 ▻ 2)
+                    ((v, lift vt (w0 ▻ 2)) :: G0[step])
+                    (Ty_hole (w0 ▻ 2) 2 ctx.in_zero)) as "IHT"; clear IHT.
+      wsimpl.
+      iPoseProof ("IHT" with "HeqG Heq1") as "-#IHT'". iRevert "IHT'". iClear "IHT".
+      iApply wp_mono. unfold _4. iIntros (w1 r1 _). wsimpl.
+    - iIntros "#HeqG #Heqt".
+      iExists (lift t2 _).
+      iModIntro. iIntros "#Heq1".
+      rewrite wp_bind.
+      iPoseProof (IHT1 (w0 ▻ 0) G0[step (R := Alloc)] (Ty_func (w0 ▻ 0) (Ty_hole (w0 ▻ 0) 0 ctx.in_zero) t0[step (R := Sub)])) as "IHT1"; clear IHT1.
+      wsimpl.
+      iPoseProof ("IHT1" with "HeqG Heq1 Heqt") as "-#IHT1'". iRevert "IHT1'". iClear "IHT1".
+      iApply wp_mono. unfold _4. iIntros (w1 r1 _). iModIntro. wsimpl.
+      iApply IHT2; wsimpl.
+  Qed.
+
+End CandidateType.
+
+Module Reconstruct.
+
+  Import Pred Pred.notations.
+  Import (hints) Sub.
+  Import ProgramLogic Pred.proofmode.
+  Import iris.proofmode.tactics.
+  Open Scope pred_scope.
+
+  Import Pred Pred.notations.
+  Import World.notations.
+
+  Lemma soundness e :
+    forall (w : World) (G : Env w),
+      ⊢ WLP w (reconstruct e G) (fun w1 r1 '(t,ee) =>
+                                   G[r1] |--ₚ e; t ~> ee).
+  Proof.
+    induction e; cbn; intros w G; unfold T, _4; wsimpl.
+    - constructor. intros ι _. pred_unfold. cbn. constructor.
+    - constructor. intros ι _. pred_unfold. cbn. constructor.
+    - rewrite wlp_bind. unfold _4. cbn.
+      iPoseProof (IHe1 w G) as "-#IH1". iRevert "IH1". clear IHe1.
+      iApply wlp_mono. iIntros (w1 r1 (t1 & e1')). cbn. iIntros "!> HT1 Heq1".
+
+      rewrite wlp_bind. unfold _4. wsimpl.
+      iPoseProof (IHe2 w1 G[r1]) as "-#IH2". iRevert "IH2". clear IHe2.
+      iApply wlp_mono. iIntros (w2 r2 (t2 & e2')). cbn. iIntros "!> HT2".
+
+      rewrite wlp_bind. unfold _4.
+      iPoseProof (IHe3 w2 G[r1 ⊙ r2]) as "-#IH3". iRevert "IH3". clear IHe3.
+      iApply wlp_mono. iIntros (w3 r3 (t3 & e3')). cbn. iIntros "!> HT3 Heq2".
+      wsimpl.
+      iStopProof. constructor. intros ι (HT1 & Heq1 & HT2 & HT3 & Heq2).
+      pred_unfold. constructor; auto.
+
+    - destruct resolve eqn:?; wsimpl.
+      constructor. intros ι _; pred_unfold.
+      constructor. now rewrite resolve_inst Heqo.
+    - rewrite wlp_bind. unfold _4. cbn.
+      iIntros "!>".
+      iPoseProof (IHe (w ▻ ctx.length w)
+                    ((s, Ty_hole (w ▻ ctx.length w) (ctx.length w) ctx.in_zero) :: G[step])) as "-#IH". iRevert "IH". clear IHe.
+      iApply wlp_mono. iIntros (w1 r1 (t1 & e1')).
+      iIntros "!> HT". wsimpl.
+      iStopProof. constructor. intros ι HT1. pred_unfold. now constructor.
+    - rewrite wlp_bind. unfold _4. cbn.
+      iPoseProof (IHe w ((s, lift t w) :: G)) as "-#IH". iRevert "IH". clear IHe.
+      iApply wlp_mono. iIntros (w1 r1 (t1 & e1')).
+      iIntros "!> HT". wsimpl.
+      iStopProof. constructor. intros ι HT1. pred_unfold.
+      now constructor.
+    - rewrite wlp_bind. unfold _4.
+      iPoseProof (IHe1 w G)
+        as "-#IH". iRevert "IH". clear IHe1.
+      iApply wlp_mono. iIntros (w1 r1 (t12 & e1')) "!> HT1".
+      rewrite wlp_bind. unfold _4.
+      iPoseProof (IHe2 w1 G[r1]) as "-#IH". iRevert "IH". clear IHe2.
+      iApply wlp_mono. iIntros (w2 r2 (t1 & e2')) "!> HT2". cbn. unfold _4. wsimpl. iIntros "!> Heq1".
+      rewrite lk_refl.
+      iStopProof. constructor. intros ι (HT1 & HT2 & Heq1). pred_unfold.
+      econstructor; eauto.
+  Qed.
+
+  Lemma completeness_aux {G e t ee} (T : G |-- e; t ~> ee) :
+    forall w0 (G0 : Env w0),
+      ⊢ liftEnv G _ =ₚ G0 →
+        WP _ (reconstruct e G0)
+          (fun w1 r01 '(t',e') => lift t w1 =ₚ t' /\ₚ S.pure ee =ₚ e')%P.
+  Proof.
+    induction T; intros w0 G0; wsimpl; unfold _4, Definitions.T.
+    - iIntros "#HeqG". rewrite wp_bind. unfold _4.
+      iPoseProof (IHT1 w0 G0 with "HeqG") as "-#IH".
+      clear IHT1. wsimpl.
+      iRevert "IH". iApply wp_mono. iIntros (w1 r1 (t1 & e1')) "!> (#Heq1 & #Heq2)". wsimpl.
+      iSplit. wsimpl.
+
+      rewrite wp_bind. unfold _4.
+      iPoseProof (IHT2 w1 G0[r1] with "HeqG") as "-#IH". clear IHT2.
+      iRevert "IH". iApply wp_mono. iIntros (w2 r2 (t2 & e2')). wsimpl.
+      iIntros "!> #Heq3 #Heq4". wsimpl.
+
+      rewrite wp_bind. unfold _4.
+      iPoseProof (IHT3 w2 G0 with "HeqG") as "-#IH". clear IHT3.
+      iRevert "IH". iApply wp_mono. iIntros (w3 r3 (t3 & e3')). wsimpl.
+      iIntros "!> #Heq5 #Heq6". wsimpl.
+      repeat iSplit; auto.
+      + admit.
+      + admit.
+
+    - constructor. intros ι. pred_unfold.
+      rewrite inst_lift_env. intros _ ->.
+      rewrite resolve_inst in H.
+      destruct resolve.
+      + injection H. clear H. intros <-.
+        cbn. now pred_unfold.
+      + discriminate H.
+    - iIntros "#HeqG".
+      iExists (lift vt _). iIntros "!> #Heq1".
+      rewrite wp_bind. unfold _4. wsimpl.
+      iPoseProof (IHT (w0 ▻ ctx.length w0) ((v, Ty_hole (w0 ▻ ctx.length w0) (ctx.length w0) ctx.in_zero) :: G0)) as "IHT".
+      wsimpl.
+      iPoseProof ("IHT" with "Heq1 HeqG") as "-#IHT'". iRevert "IHT'". iClear "IHT".
+      iApply wp_mono. iIntros (w1 r1 (t1 & e1')) "!> (#Heq2 & #Heq3)". wsimpl.
+      repeat iSplit; auto.
+      admit.
+
+    - admit.
+    - admit.
+  Admitted.
+
+  Lemma wp_impl {A w} (m : FreeM A w) (P : □⁺(A -> Pred) w) (Q : Pred w) :
+    (WP _ m P ->ₚ Q) ⊣⊢ₚ WLP _ m (fun w1 r01 a1 => P w1 r01 a1 ->ₚ Ext Q r01)%P.
+  Proof.
+    (* unfold Ext, bientails, implₚ. revert P Q. *)
+    (* induction m; cbn; unfold T, _4, Basics.impl. *)
+    (* - easy. *)
+    (* - intros. intuition. *)
+    (* - split; intuition. now apply IHm. *)
+    (* - intros. specialize (IHm (_4 P step) (Ext Q step)). *)
+    (*   cbn. split. *)
+    (*   + intros HQ t. specialize (IHm (env.snoc ι _ t)). *)
+    (*     apply IHm. intros Hwp. apply HQ. exists t. apply Hwp. *)
+    (*   + intros Hwlp (t & Hwp). specialize (Hwlp t). *)
+    (*     apply IHm in Hwlp; auto. *)
+  Admitted.
+
+  Theorem correctness e :
+    forall w (G : Env w) Q (RQ : ProperPost Q),
+      WP _ (reconstruct e G) Q ⊣⊢ₚ
+      ∃ₚ t : Ty w, ∃ₚ ee : Expr w, TPB G e t ee /\ₚ T Q (t,ee).
+  Proof.
+    (* intros w G Q RQ ι. unfold T. split. *)
+    (* - apply wp_impl. generalize (@soundness e w ι G). apply wlp_monotonic. *)
+    (*   intros w1 r01 [t e'] ι1 (Heq & HT) HQ. subst. cbn. *)
+    (*   exists (lift (inst t ι1) _). *)
+    (*   exists (fun _ => inst e' ι1). cbn. *)
+    (*   rewrite inst_lift. cbn. split. apply HT. unfold T. *)
+    (*   change (Ext (T Q (lift (inst t ι1) w, fun _ : Assignment w => inst e' ι1)) r01 ι1). *)
+    (*   specialize (RQ _ r01 (lift (inst t ι1) w, fun _ : Assignment w => inst e' ι1) (t, e') ι1). *)
+    (*   unfold entails, implₚ in RQ. cbn in RQ. *)
+    (*   rewrite inst_persist_ty, inst_lift in RQ. *)
+    (*   specialize (RQ eq_refl). intuition. *)
+    (* - intros (t & e' & HT & HQ). *)
+    (*   generalize (@completeness_aux e w G ι (inst G ι) eq_refl (inst t ι) (inst e' ι) HT). *)
+    (*   apply wp_monotonic. intros w1 r01 [t1 e1'] ι1 (Heq & Heqt). subst. *)
+    (*   specialize (RQ _ r01 (t,e') (t1,e1') ι1). cbn in RQ. *)
+    (*   rewrite inst_persist_ty, Heqt in RQ. *)
+    (*   apply RQ; auto. f_equal. clear. *)
+    (*   admit. *)
+  Admitted.
+
+End Reconstruct.
 
 Module StrongMonotonicity.
 
@@ -355,10 +1245,10 @@ Module StrongMonotonicity.
   Definition M (A : TYPE) : TYPE :=
     Option (Diamond Sub A).
 
-  Definition pure {A} : ⊢ A -> M A :=
+  Definition pure {A} : ⊢ʷ A -> M A :=
     fun w a => Some (existT w (refl, a)).
 
-  Definition bind {A B} : ⊢ M A -> □ˢ(A -> (M B)) -> M B :=
+  Definition bind {A B} : ⊢ʷ M A -> □ˢ(A -> (M B)) -> M B :=
     fun w m f =>
       '(existT w1 (r1,a1)) <- m;;
       '(existT w2 (r2,b2)) <- f w1 r1 a1;;
@@ -368,12 +1258,12 @@ Module StrongMonotonicity.
     '(w';(r,a)) <- m ;;
     Some (existT w' (step ⊙ r, a)).
 
-  Definition mgu : ⊢ Ty -> Ty -> M Unit :=
+  Definition mgu : ⊢ʷ Ty -> Ty -> M Unit :=
     fun w t1 t2 =>
       '(w;(r,u)) <- Variant1.mgu t1 t2 ;;
       Some (w; (Sub.triangular r, u)).
 
-  Definition WLP {A} : ⊢ M A -> □ˢ(A -> PROP) -> PROP :=
+  Definition WLP {A} : ⊢ʷ M A -> □ˢ(A -> PROP) -> PROP :=
     fun w m P => option.wlp (fun '(w;(r,a)) => P w r a) m.
 
   Lemma wlp_pure {A w} (a : A w) (p : □ˢ(A -> PROP) w) :
@@ -417,7 +1307,7 @@ Module StrongMonotonicity.
     apply pq.
   Qed.
 
-  Definition WP {A} : ⊢ M A -> □ˢ(A -> PROP) -> PROP :=
+  Definition WP {A} : ⊢ʷ M A -> □ˢ(A -> PROP) -> PROP :=
     fun w m P => option.wp (fun '(w;(r,a)) => P w r a) m.
 
   Lemma wp_pure {A w} (a : A w) (p : □ˢ(A -> PROP) w) :
@@ -623,373 +1513,6 @@ Module StrongMonotonicity.
 
 End StrongMonotonicity.
 
-(* Focus on the constraint generation only, forget about solving constraints
-   and any semantic values. Also try to pass the type as an input instead of
-   an output, i.e. checking instead of synthesizing. *)
-Module ConstraintsOnly.
-
-  Import World.notations.
-  Import option.notations.
-  Import Unification.
-
-  #[local] Set Implicit Arguments.
-  #[local] Arguments step : simpl never.
-
-  Module C.
-
-    Import Pred Pred.notations.
-    Import (hints) Sub.
-
-    Inductive CStr (w : World) : Type :=
-    | False
-    | Eq (t1 t2 : Ty w)
-    | And (C1 C2 : CStr w)
-    | Ex {x} (C : CStr (w ▻ x)).
-    #[global] Arguments False {w}.
-    #[global] Arguments Ex [w] x C.
-
-    Definition denote : ⊢ CStr -> Assignment -> PROP :=
-      fix den {w} C ι {struct C} : Prop :=
-        match C with
-        | False     => Logic.False
-        | Eq t1 t2  => inst t1 ι = inst t2 ι
-        | And C1 C2 => den C1 ι /\ den C2 ι
-        | Ex x C    => exists t, den C (env.snoc ι x t)
-        end.
-
-  End C.
-  Export C (CStr).
-
-  Notation "C1 /\ C2" := (C.And C1 C2).
-  Notation "t1 == t2" := (C.Eq t1 t2) (at level 80).
-  Notation "∃ n , C" := (C.Ex n C) (at level 80, right associativity, format "∃ n ,  C").
-
-  Fixpoint check (e : expr) : ⊢ Env -> Ty -> CStr :=
-    fun (w : World) (G : Env w) (tr : Ty w) =>
-      match e with
-      | v_true => tr == Ty_bool w
-      | v_false => tr == Ty_bool w
-      | e_if e1 e2 e3 =>
-          check e1 G (Ty_bool w) /\
-          check e2 G tr /\
-          check e3 G tr
-      | e_var s =>
-          match resolve s G with
-          | Some a => tr == a
-          | None => C.False
-          end
-      | e_absu x e =>
-          ∃1, ∃2,
-            let G'  := <{ G ~ step ⊙ step }> in
-            let tr' := <{ tr ~ step ⊙ step }> in
-            let α1  := Ty_hole (w ▻ 1 ▻ 2) 1 (ctx.in_succ ctx.in_zero) in
-            let α2  := Ty_hole (w ▻ 1 ▻ 2) 2 ctx.in_zero in
-            (tr' == Ty_func _ α1 α2) /\
-            check e ((x, α1) :: G') α2
-      | e_abst x xt e =>
-          ∃2,
-            let G'  := <{ G ~ step }> in
-            let tr' := <{ tr ~ step }> in
-            let α1  := lift xt _ in
-            let α2  := Ty_hole (w ▻ 2) 2 ctx.in_zero in
-            (tr' == Ty_func _ α1 α2) /\
-            check e ((x, α1) :: G') α2
-      | e_app e1 e2 =>
-          ∃0,
-            let G'  := <{ G ~ step }> in
-            let tr' := <{ tr ~ step }> in
-            let α   := Ty_hole (w ▻ 0) 0 ctx.in_zero in
-            check e1 G' (Ty_func _ α tr') /\
-            check e2 G' α
-      end.
-
-  Lemma soundness e :
-    forall (w : World) G t (ι : Assignment w),
-      C.denote (check e G t) ι ->
-      exists ee, inst G ι |-- e ; inst t ι ~> ee.
-  Proof.
-    induction e; cbn; intros w G tr ι.
-    - intros ->. eexists. constructor.
-    - intros ->. eexists. constructor.
-    - intros (H1 & H2 & H3).
-      specialize (IHe1 _ _ _ _ H1). clear H1. destruct IHe1 as (e1' & HT1).
-      specialize (IHe2 _ _ _ _ H2). clear H2. destruct IHe2 as (e2' & HT2).
-      specialize (IHe3 _ _ _ _ H3). clear H3. destruct IHe3 as (e3' & HT3).
-      eexists. constructor; eauto.
-    - destruct resolve eqn:?; cbn; intros Heq; [|contradiction].
-      eexists. constructor. now rewrite resolve_inst, Heqo, Heq.
-    - intros (t1 & t2 & H1 & H2).
-      specialize (IHe _ _ _ _ H2). clear H2.
-      destruct IHe as (e1' & HT). cbn in HT.
-      rewrite ?inst_lift, ?inst_persist_env, ?inst_persist_ty, ?inst_trans, ?inst_step_snoc in *.
-      rewrite H1. clear H1.
-      eexists. constructor. eauto.
-    - intros (t1 & H1 & H2).
-      specialize (IHe _ _ _ _ H2). clear H2.
-      destruct IHe as (e' & HT). cbn in HT.
-      rewrite ?inst_lift, ?inst_persist_env, ?inst_persist_ty, ?inst_trans, ?inst_step_snoc in *.
-      rewrite H1. clear H1.
-      eexists. constructor. eauto.
-    - intros (t1 & H1 & H2).
-      specialize (IHe1 _ _ _ _ H1). clear H1. destruct IHe1 as (e1' & HT1).
-      specialize (IHe2 _ _ _ _ H2). clear H2. destruct IHe2 as (e2' & HT2).
-      exists (e_app e1' e2').
-      cbn in HT1, HT2.
-      rewrite ?inst_lift, ?inst_persist_env, ?inst_persist_ty, ?inst_trans, ?inst_step_snoc in *.
-      econstructor; eauto.
-  Qed.
-
-  Lemma completeness_aux {G e t ee} (T : G |-- e; t ~> ee) :
-    forall (w0 : World) (ι0 : Assignment w0) (G0 : Env w0) (t0 : Ty w0),
-      G = inst G0 ι0 -> t = inst t0 ι0 -> C.denote (check e G0 t0) ι0.
-  Proof.
-    induction T; cbn; intros w0 ι0 G0 t0 ? ?; subst.
-    - auto.
-    - auto.
-    - intuition.
-    - rewrite resolve_inst in H.
-      destruct resolve; [|discriminate].
-      now injection H.
-    - exists vt, t. rewrite H0. split.
-      + now rewrite inst_persist_ty, inst_trans, !inst_step_snoc.
-      + apply IHT; cbn; [|easy].
-        now rewrite inst_persist_env, inst_trans, !inst_step_snoc.
-    - exists t. split.
-      + now rewrite inst_lift, inst_persist_ty, inst_step_snoc.
-      + apply IHT; cbn; [|easy].
-        now rewrite inst_lift, inst_persist_env, inst_step_snoc.
-    - exists t2. split.
-      + apply IHT1; cbn.
-        * now rewrite inst_persist_env, inst_step_snoc.
-        * now rewrite inst_persist_ty, inst_step_snoc.
-      + apply IHT2; cbn; [|easy].
-        now rewrite inst_persist_env, inst_step_snoc.
-  Qed.
-
-  Corollary completeness G e t ee (T : G |-- e ; t ~> ee) :
-    C.denote (check e (liftEnv G _) (lift t _)) env.nil.
-  Proof.
-    eapply completeness_aux; eauto.
-    - now rewrite inst_lift_env.
-    - now rewrite inst_lift.
-  Qed.
-
-End ConstraintsOnly.
-
-Module CandidateType.
-
-  Import World.notations.
-
-  #[local] Set Implicit Arguments.
-  #[local] Arguments step : simpl never.
-  #[local] Arguments step : simpl never.
-
-  Local Notation "[ ω ] x <- ma ;; mb" :=
-    (bind (R := Alloc) ma (fun _ ω x => mb))
-      (at level 80, x at next level,
-        ma at next level, mb at level 200,
-        right associativity).
-
-  Local Notation "∃ n , m" :=
-    (Bind_Exists_Free _ _ n m)
-      (at level 80, right associativity, format "∃ n ,  m").
-
-  Notation "t1 == t2 //\ m" := (Bind_AssertEq_Free _ _ t1 t2 m) (at level 70).
-
-  Fixpoint check (e : expr) : ⊢ Env -> Ty -> FreeM Unit :=
-    fun w G tr =>
-      match e with
-      | v_true => Bind_AssertEq_Free Unit w tr (Ty_bool w) (Ret_Free Unit w tt)
-      | v_false => Bind_AssertEq_Free Unit w tr (Ty_bool w) (Ret_Free Unit w tt)
-      | e_if e0 e1 e2 =>
-        [r1] _ <- check e0 G (Ty_bool w)   ;;
-        [r2] _ <- check e1 <{ G ~ r1 }> <{ tr ~ r1 }> ;;
-        check e2 <{ G ~ r1 ⊙ r2 }> <{ tr ~ r1 ⊙ r2 }>
-      | e_var s =>
-        match resolve s G with
-        | Some a => Bind_AssertEq_Free Unit w tr a (Ret_Free Unit w tt)
-        | None => Fail_Free Unit w
-        end
-      | e_absu s e0 =>
-        ∃1, ∃2,
-          let tr' := <{ tr ~ step ⊙ step }> in
-          let α1  := Ty_hole _ 1 (ctx.in_succ ctx.in_zero) in
-          let α2  := Ty_hole _ 2 ctx.in_zero in
-          tr' == Ty_func _ α1 α2 //\
-          check e0 ((s, α1) :: <{ G ~ step ⊙ step }>) α2
-
-      | e_abst s t e0 =>
-        ∃2,
-          let tr' := <{ tr ~ step }> in
-          let α1  := lift t (w ▻ 2) in
-          let α2  := Ty_hole (w ▻ 2) 2 ctx.in_zero in
-          tr' == Ty_func (w ▻ 2) α1 α2 //\
-          check e0 ((s, α1) :: <{ G ~ step }>) α2
-      | e_app e0 e1 =>
-        ∃0,
-          let α := Ty_hole (w ▻ 0) 0 ctx.in_zero in
-          [r1] _ <- check e0 <{ G ~ step }> (Ty_func _ α <{ tr ~ step }>) ;;
-                    check e1 <{ G ~ step ⊙ r1 }> <{ α ~ r1 }>
-  end.
-
-  Lemma lookup_inst {w1 w2 : World} (r : Alloc w1 w2) (ι : Assignment w2) {x} (i : x ∈ w1) :
-    env.lookup (inst r ι) i = env.lookup ι <{ i ~ r }>.
-  Proof. induction r. reflexivity. cbn. rewrite <- IHr. now destruct env.view. Qed.
-
-  Lemma completeness_aux {G e t ee} (T : G |-- e; t ~> ee) :
-    forall (w0 : World) (ι0 : Assignment w0) (G0 : Env w0) (t0 : Ty w0),
-      G = inst G0 ι0 -> t = inst t0 ι0 ->
-      WP (check e G0 t0) (fun w1 r01 _ ι1 => ι0 = inst r01 ι1)%type ι0.
-  Proof.
-    Set Printing Depth 17.
-    induction T; cbn; intros w0 ι0 G0 t0 ? ?; subst.
-    + easy.
-    + easy.
-    + rewrite wp_bind. specialize (IHT1 w0 ι0 G0 (Ty_bool w0) eq_refl eq_refl).
-      revert IHT1.
-      apply wp_monotonic. intros w1 r1 _ ι1 Hι0.
-      rewrite wp_bind.
-      specialize (IHT2 w1 ι1 <{ G0 ~ r1 }> <{ t0 ~ r1}>).
-      rewrite inst_persist_env in IHT2.
-      rewrite inst_persist_ty in IHT2.
-      rewrite Hι0 in IHT2.
-      specialize (IHT2 eq_refl eq_refl).
-      revert IHT2. apply wp_monotonic. intros w2 r2 _ ι2 Hι1.
-      specialize (IHT3 w2 ι2 <{ G0 ~ r1 ⊙ r2 }> <{ t0 ~ r1 ⊙ r2 }>).
-      rewrite inst_persist_env in IHT3.
-      rewrite inst_persist_ty in IHT3.
-      rewrite Hι0, Hι1, inst_trans in IHT3.
-      specialize (IHT3 eq_refl eq_refl).
-      revert IHT3. apply wp_monotonic. unfold _4.
-      intros w3 r3 _ ι3 Hι2.
-      now rewrite Hι0, Hι1, Hι2, !inst_trans.
-    + rewrite resolve_inst in H. destruct resolve; cbn in *; now inversion H.
-    + exists vt. exists t.
-      rewrite inst_persist_ty, inst_trans, !inst_step_snoc.
-      split; [easy|].
-      specialize (IHT (w0 ▻ 1 ▻ 2)
-                      (env.snoc (env.snoc ι0 1 vt) 2 t)
-                      ((v, Ty_hole (w0 ▻ 1 ▻ 2) 1 (ctx.in_succ ctx.in_zero)) :: <{ G0 ~ step ⊙ step }>)
-                      (Ty_hole (w0 ▻ 1 ▻ 2) 2 ctx.in_zero)).
-      cbn in IHT. rewrite inst_persist_env, inst_trans, !inst_step_snoc in IHT.
-      specialize (IHT eq_refl eq_refl).
-      revert IHT. apply wp_monotonic. intros. hnf.
-      now rewrite !inst_trans, <- H.
-    + exists t.
-      rewrite inst_persist_ty, inst_lift, inst_step_snoc, H0.
-      split; [easy|].
-      specialize (IHT (w0 ▻ 2)
-                      (env.snoc ι0 2 t)
-                      ((v, lift vt (w0 ▻ 2)) :: <{ G0 ~ step }>)
-                      (Ty_hole (w0 ▻ 2) 2 ctx.in_zero)).
-      cbn in IHT.
-      rewrite inst_lift in IHT.
-      rewrite inst_persist_env in IHT.
-      rewrite inst_step_snoc in IHT.
-      specialize (IHT eq_refl eq_refl).
-      revert IHT. apply wp_monotonic. intros. hnf.
-      now rewrite inst_trans, <- H.
-    + exists t2.
-      rewrite wp_bind.
-      specialize (IHT1 (w0 ▻ 0)
-                       (env.snoc ι0 0 t2)
-                       <{ G0 ~ step }>
-                       (Ty_func (w0 ▻ 0) (Ty_hole (w0 ▻ 0) 0 ctx.in_zero) <{ t0 ~ step }>)).
-      cbn in IHT1.
-      rewrite inst_persist_env in IHT1.
-      rewrite inst_persist_ty in IHT1.
-      rewrite inst_step_snoc in IHT1.
-      specialize (IHT1 eq_refl eq_refl).
-      revert IHT1. apply wp_monotonic. intros.
-      specialize (IHT2 _ ι1 <{ G0 ~ step ⊙ r1 }> (Ty_hole w1 0 <{ ctx.in_zero ~ r1 }>)).
-      cbn in IHT2.
-      rewrite inst_persist_env in IHT2.
-      rewrite inst_trans in IHT2.
-      rewrite <- lookup_inst, <- H in IHT2.
-      specialize (IHT2 eq_refl eq_refl).
-      revert IHT2. apply wp_monotonic. intros. hnf.
-      now rewrite !inst_trans, <- H0, <- H.
-  Qed.
-
-  Lemma soundness e :
-    forall (w0 : World) (ι0 : Assignment w0) (G0 : Env w0) (t0 : Ty w0),
-      WLP (check e G0 t0)
-          (fun w1 r01 _ ι1 => ι0 = inst r01 ι1 /\
-                       exists ee, inst G0 ι0 |-- e ; inst t0 ι0 ~> ee)
-          ι0.
-  Proof.
-    induction e; cbn; intros.
-    - split. auto. rewrite H. eexists. constructor.
-    - split. auto. rewrite H. eexists. constructor.
-    - rewrite wlp_bind. specialize (IHe1 _ ι0 G0 (Ty_bool w0)).
-      revert IHe1. apply wlp_monotonic. intros.
-      rewrite wlp_bind. specialize (IHe2 _ ι1 <{ G0 ~ r1 }> <{ t0 ~ r1}>).
-      revert IHe2. apply wlp_monotonic. intros.
-      specialize (IHe3 _ ι2 <{ G0 ~ r1 ⊙ r0 }> <{ t0 ~ r1 ⊙ r0 }>).
-      revert IHe3. apply wlp_monotonic. intros.
-      hnf. destruct H1, H0, H. subst.
-      rewrite ?inst_persist_env,
-              ?inst_persist_ty,
-              ?inst_trans in *.
-      split; [easy|].
-      firstorder.
-      exists (e_if x0 x1 x).
-      now constructor.
-    - destruct (resolve s G0) eqn:?; [|easy].
-      intros Heqt. split; [easy|].
-      exists (e_var s). constructor.
-      rewrite resolve_inst, Heqo. cbn. congruence.
-    - specialize (IHe _ (env.snoc (env.snoc ι0 1 t) 2 t1)
-                        ((s, Ty_hole (w0 ▻ 1 ▻ 2) 1 (ctx.in_succ ctx.in_zero))
-                             :: <{ G0 ~ step ⊙ step }>)
-                        (Ty_hole (w0 ▻ 1 ▻ 2) 2 ctx.in_zero)).
-      revert IHe. apply wlp_monotonic. unfold _4. cbn.
-      intros ? ? _ ? (Hι1 & e' & IHe).
-      rewrite
-        ?inst_persist_env,
-        ?inst_persist_ty,
-        ?inst_trans, <- ?Hι1, ?inst_step_snoc in *.
-      split; [easy|].
-      exists (e_abst s t e').
-      rewrite H.
-      now constructor.
-    - specialize (IHe _ (env.snoc ι0 2 t1)
-                        ((s, lift t (w0 ▻ 2)) :: <{ G0 ~ step }>)
-                        (Ty_hole (w0 ▻ 2) 2 ctx.in_zero)).
-      revert IHe. apply wlp_monotonic. intros. hnf.
-      destruct H0 as (Heq & e' & Ht). split. now rewrite inst_trans, <- Heq.
-      exists (e_abst s t e'). cbn in *.
-      Set Printing Depth 50.
-      rewrite
-        ?inst_persist_env,
-        ?inst_persist_ty,
-        ?inst_trans, ?inst_step_snoc in *.
-      rewrite H, inst_lift in *.
-      now constructor.
-    - rewrite wlp_bind.
-      specialize (IHe1 _ (env.snoc ι0 0 t)
-                        <{ G0 ~ step }>
-                        (Ty_func (w0 ▻ 0)
-                           (Ty_hole (w0 ▻ 0) 0 ctx.in_zero)
-                           <{ t0 ~ step }>)).
-      revert IHe1. apply wlp_monotonic. intros.
-      specialize (IHe2 _ ι1 <{ G0 ~ step ⊙ r1 }> (lk r1 ctx.in_zero)).
-      revert IHe2. apply wlp_monotonic. intros. hnf.
-      destruct H0 as (Hι1 & e2' & Hte2), H as (Hsnoc & e1' & Hte1).
-      split. now rewrite ?inst_trans, <- Hι1, <- Hsnoc, inst_step.
-      exists (e_app e1' e2').
-      constructor 7 with t;
-      rewrite
-        ?inst_persist_env,
-        ?inst_persist_ty,
-        ?inst_trans, ?inst_step_snoc, ?inst_step, <- ?Hsnoc in *; cbn in *;
-      rewrite ?lookup_inst, <- ?Hsnoc in *.
-      + now rewrite inst_persist_ty, inst_step_snoc in Hte1.
-      + now rewrite <- lookup_inst, <- Hsnoc in Hte2.
-  Qed.
-
-End CandidateType.
-
 Module ProofWorlds.
 
   Import World.notations.
@@ -1009,7 +1532,7 @@ Module ProofWorlds.
 
   #[local] Notation "t1 == t2 //\ m" := (Bind_AssertEq_Free _ _ t1 t2 m) (at level 70).
 
-  Fixpoint check (e : expr) : ⊢ Env -> Ty -> FreeM Unit :=
+  Fixpoint check (e : expr) : ⊢ʷ Env -> Ty -> FreeM Unit :=
     fun w G tr =>
       match e with
       | v_true => Bind_AssertEq_Free Unit w tr (Ty_bool w) (Ret_Free Unit w tt)
@@ -1168,437 +1691,3 @@ Module ProofWorlds.
   Proof. Admitted.
 
 End ProofWorlds.
-
-
-Section Correctness.
-
-  Import Pred Pred.notations.
-  Import World.notations.
-
-  Lemma soundness e :
-    forall (w0 : World) (ι0 : Assignment w0) (G0 : Env w0),
-      WLP (reconstruct e G0)
-          (fun w1 r01 '(t,ee) ι1 => ι0 = inst r01 ι1 /\
-                                   inst G0 ι0 |-- e ; inst t ι1 ~> inst ee ι1)
-          ι0.
-  Proof.
-    induction e; cbn; intros.
-    - repeat constructor.
-    - repeat constructor.
-    - rewrite wlp_bind. specialize (IHe1 _ ι0 G0).
-      revert IHe1. apply wlp_monotonic. intros w1 r1 v1 ι1 Hv1.
-      destruct v1 eqn:? in Hv1. destruct Hv1. intro.
-      unfold T.
-      rewrite wlp_bind. specialize (IHe2 _ ι1 <{ G0 ~ r1 ⊙ refl }>).
-      revert IHe2. apply wlp_monotonic. intros w2 r2 v2 ι2 Hv2.
-      destruct v2 eqn:? in Hv2. destruct Hv2.
-      rewrite wlp_bind.
-      specialize (IHe3 _ ι2 <{ G0 ~ r1 ⊙ refl ⊙ r2 }>).
-      revert IHe3. apply wlp_monotonic. intros w3 r3 v3 ι3 Hv3.
-      destruct v3 eqn:? in Hv3. destruct Hv3. intro.
-      hnf.
-      rewrite ?inst_persist_env,
-              ?inst_persist_ty,
-              ?inst_trans in *. cbn.
-      split. now rewrite <- H4, <- H2, <- H.
-      constructor 3.
-      + rewrite Heqp. cbn.
-        rewrite ?inst_trans. cbn.
-        rewrite <- H4, <- H2.
-        rewrite Heqp in H1. cbn in H1.
-        rewrite H1 in H0. unfold inst, inst_sem in H0.
-        apply H0.
-      + rewrite Heqp0. cbn. rewrite <- H4. rewrite inst_trans. cbn. rewrite <- H4. cbn in H3. rewrite <- H in H3. unfold inst, inst_sem in H3. apply H3.
-      + rewrite Heqp0, Heqp1. cbn. rewrite <- H4. cbn in H5. rewrite <- H2, <- H in H5. rewrite Heqp0, Heqp1 in H6. cbn in H6. rewrite <- H4 in H6. rewrite H6. apply H5.
-    - destruct (resolve s G0) eqn:?; [|easy].
-      cbn. unfold T. split. auto. constructor.
-      rewrite resolve_inst, Heqo. cbn. congruence.
-    - unfold T, _4.
-      rewrite wlp_bind.
-      rewrite trans_refl_r.
-      specialize (IHe _ (env.snoc ι0 (ctx.length w0) t) ((s,
-         Ty_hole (w0 ▻ ctx.length w0) (ctx.length w0)
-           ctx.in_zero) :: <{ G0 ~ step }>)).
-      revert IHe. apply wlp_monotonic. intros w1 r1 v1 ι1 Hv1.
-      destruct v1 eqn:? in Hv1. destruct Hv1. cbn.
-      unfold T, _4.
-      rewrite ?inst_persist_env,
-              ?inst_persist_ty,
-              ?inst_trans in *. cbn.
-      rewrite <- H. split. auto.
-      constructor.
-      cbn in H0. rewrite <- CandidateType.lookup_inst. rewrite <- H. cbn.
-      rewrite Heqp. cbn.
-      rewrite ?inst_persist_env,
-              ?inst_persist_ty,
-              ?inst_trans in *. cbn in *.
-      apply H0.
-    - rewrite wlp_bind.
-      specialize (IHe _ ι0 ((s, lift t w0) :: G0)).
-      revert IHe. apply wlp_monotonic. intros w1 r1 v1 ι1 Hv1.
-      destruct v1 eqn:? in Hv1. destruct Hv1. cbn.
-      unfold T, _4.
-      split. rewrite inst_trans. cbn. now rewrite <- H.
-      rewrite Heqp. cbn.
-      rewrite ?inst_persist_ty, ?inst_lift.
-      constructor 6. cbn in H0.
-      now rewrite ?inst_lift in H0.
-    - unfold T, _4. rewrite wlp_bind.
-      rewrite trans_refl_r.
-      specialize (IHe2 _ (env.snoc ι0 (ctx.length w0) t) <{ G0 ~ step }>).
-      revert IHe2. apply wlp_monotonic. intros w1 r1 v1 ι1 Hv1.
-      destruct v1 eqn:? in Hv1. destruct Hv1. cbn.
-      rewrite wlp_bind.
-      specialize (IHe1 _ ι1 <{ G0 ~ alloc.fresh w0 (ctx.length w0) w1 r1 }>).
-      revert IHe1. apply wlp_monotonic. intros w2 r2 v2 ι2 Hv2.
-      destruct v2 eqn:? in Hv2. destruct Hv2. cbn.
-      intro.
-      unfold T, _4.
-      rewrite ?inst_persist_env,
-              ?inst_persist_ty,
-              ?inst_trans in *. cbn in *.
-      rewrite Heqp, Heqp0, <- H1 in H3. cbn in H3.
-      rewrite <- H1, <- H. cbn. split. auto.
-      constructor 7 with (inst t0 ι1). rewrite <- H in H2. cbn in H2.
-      rewrite <- CandidateType.lookup_inst in H3.
-      rewrite <- H1 in H3.
-      rewrite Heqp0. cbn.
-      rewrite <- CandidateType.lookup_inst.
-      rewrite ?inst_trans. cbn.
-      rewrite <- H1, <- H. cbn.
-      rewrite H3 in H2.
-      rewrite <- CandidateType.lookup_inst in H2. rewrite <- H in H2. cbn in H2.
-      apply H2.
-      rewrite Heqp. cbn. rewrite ?inst_trans. cbn. rewrite <- H1.
-      apply H0.
-  Qed.
-
-  Lemma completeness_aux e :
-    forall (w0 : World) (G0 : Env w0) (ι0 : Assignment w0),
-    forall {G}, G = inst G0 ι0 ->
-      forall {t ee} (T : G |-- e; t ~> ee),
-      WP (reconstruct e G0) (fun w1 r01 '(t',ee) ι1 =>
-                                             ι0 = inst r01 ι1 /\
-                                             t = inst t' ι1) ι0.
-  Proof.
-    intros. revert w0 ι0 G0 H.
-    induction T; cbn; intros w0 ι0 G0 ?; subst.
-    + easy.
-    + easy.
-    + rewrite wp_bind. specialize (IHT1 w0 ι0 G0 eq_refl).
-      revert IHT1. apply wp_monotonic. intros w1 r1 v1 ι1 Hv1.
-      cbn. destruct v1 eqn:? in Hv1. destruct Hv1. split. now rewrite H0, Heqp.
-      unfold T.
-      rewrite wp_bind.
-      specialize (IHT2 _ ι1 <{ G0 ~ r1 ⊙ refl }>).
-      rewrite inst_persist_env in IHT2.
-      rewrite inst_trans in IHT2.
-      cbn in IHT2.
-      rewrite <- H in IHT2.
-      specialize (IHT2 eq_refl).
-      revert IHT2. apply wp_monotonic. intros w2 r2 v2 ι2 Hv2.
-      destruct v2 eqn:? in Hv2. destruct Hv2.
-      rewrite wp_bind.
-      specialize (IHT3 _ ι2 <{ G0 ~ r1 ⊙ refl ⊙ r2 }>).
-      rewrite inst_persist_env in IHT3.
-      rewrite inst_trans in IHT3.
-      cbn in IHT3.
-      rewrite <- H1, <- H in IHT3.
-      specialize (IHT3 eq_refl).
-      revert IHT3. apply wp_monotonic. intros w3 r3 v3 ι3 Hv3.
-      destruct v3 eqn:? in Hv3. destruct Hv3. cbn.
-      rewrite Heqp0, Heqp1. cbn.
-      rewrite inst_persist_ty, <- H3.
-      split. now rewrite <- H2, <- H4.
-      unfold T. hnf.
-      rewrite ?inst_persist_ty,
-              ?inst_trans. cbn.
-      now rewrite <- H3, <- H2, <- H1, <- H.
-    + rewrite resolve_inst in H. destruct resolve; cbn in *; now inversion H.
-    + exists vt.
-      unfold Definitions.T, _4.
-      rewrite wp_bind.
-      specialize (IHT _ (env.snoc ι0 (ctx.length w0) vt)
-                        ((v, Ty_hole (w0 ▻ ctx.length w0) (ctx.length w0) ctx.in_zero)
-                           :: <{ G0 ~ step ⊙ refl }>)).
-      cbn in IHT.
-      rewrite inst_persist_env in IHT.
-      cbn in IHT.
-      specialize (IHT eq_refl).
-      revert IHT. apply wp_monotonic. intros w1 r1 v1 ι1 Hv1. cbn.
-      unfold Definitions.T, _4. cbn.
-      destruct v1 eqn:? in Hv1. destruct Hv1.
-      split.
-      rewrite inst_trans. cbn. now rewrite <- H.
-      rewrite Heqp. cbn.
-      now rewrite <- H0, <- CandidateType.lookup_inst, <- H.
-    + rewrite wp_bind.
-      specialize (IHT _ ι0 ((v, lift vt w0) :: G0)).
-      cbn in IHT.
-      rewrite inst_lift in IHT.
-      specialize (IHT eq_refl).
-      revert IHT. apply wp_monotonic. intros w1 r1 v1 ι1 Hv1. cbn.
-      unfold Definitions.T, _4. cbn.
-      destruct v1 eqn:? in Hv1. destruct Hv1.
-      split.
-      rewrite inst_trans. cbn. now rewrite H.
-      rewrite inst_persist_ty. rewrite inst_lift.
-      now rewrite Heqp, H0.
-    + exists t1.
-      unfold Definitions.T, _4. cbn.
-      rewrite wp_bind.
-      specialize (IHT2 _ (env.snoc ι0 (ctx.length w0) t1) <{ G0 ~ step }>).
-      cbn in IHT2.
-      rewrite inst_persist_env in IHT2.
-      cbn in IHT2.
-      specialize (IHT2 eq_refl).
-      revert IHT2. apply wp_monotonic. intros w1 r1 v1 ι1 Hv1. cbn.
-      destruct v1 eqn:? in Hv1. destruct Hv1.
-      rewrite wp_bind.
-      specialize (IHT1 _ ι1 <{ G0 ~ alloc.fresh w0 (ctx.length w0) w1 r1 }>).
-      rewrite inst_persist_env in IHT1. cbn in IHT1.
-      Set Printing Depth 50.
-      rewrite <- H in IHT1. cbn in IHT1.
-      specialize (IHT1 eq_refl).
-      revert IHT1. apply wp_monotonic. intros w2 r2 v2 ι2 Hv2. cbn.
-      destruct v2 eqn:? in Hv2. destruct Hv2.
-      split.
-      - rewrite Heqp0. cbn.
-        rewrite <- H2, inst_persist_ty, Heqp, <- H1. cbn.
-        now rewrite <- H0,
-                    -> assoc_persist,
-                    <- CandidateType.lookup_inst,
-                    -> inst_trans,
-                    <- H1,
-                    <- H.
-      - unfold Definitions.T, _4. cbn.
-        rewrite ?inst_trans. cbn.
-        rewrite <- H1, <- H. cbn.
-        rewrite <- ?CandidateType.lookup_inst,
-                -> ?inst_trans. cbn.
-        now rewrite <- H1, <- H.
-  Qed.
-
-  Lemma wp_impl {A w} (m : FreeM A w) (P : □⁺(A -> Pred) w) (Q : Pred w) :
-    (WP m P ->ₚ Q) ⊣⊢ₚ WLP m (fun w1 r01 a1 => P w1 r01 a1 ->ₚ Ext Q r01)%P.
-  Proof.
-    unfold Ext, bientails, implₚ. revert P Q.
-    induction m; cbn; unfold T, _4, Basics.impl.
-    - easy.
-    - intros. intuition.
-    - split; intuition. now apply IHm.
-    - intros. specialize (IHm (_4 P step) (Ext Q step)).
-      cbn. split.
-      + intros HQ t. specialize (IHm (env.snoc ι _ t)).
-        apply IHm. intros Hwp. apply HQ. exists t. apply Hwp.
-      + intros Hwlp (t & Hwp). specialize (Hwlp t).
-        apply IHm in Hwlp; auto.
-  Qed.
-
-  Theorem correctness e :
-    forall w (G : Env w) Q (RQ : ProperPost Q),
-      WP (reconstruct e G) Q ⊣⊢ₚ
-      ∃ₚ t ∶ Ty w, ∃ₚ ee ∶ Expr w, TPB G e t ee /\ₚ T Q (t,ee).
-  Proof.
-    intros w G Q RQ ι. unfold T. split.
-    - apply wp_impl. generalize (@soundness e w ι G). apply wlp_monotonic.
-      intros w1 r01 [t e'] ι1 (Heq & HT) HQ. subst. cbn.
-      exists (lift (inst t ι1) _).
-      exists (fun _ => inst e' ι1). cbn.
-      rewrite inst_lift. cbn. split. apply HT. unfold T.
-      change (Ext (T Q (lift (inst t ι1) w, fun _ : Assignment w => inst e' ι1)) r01 ι1).
-      specialize (RQ _ r01 (lift (inst t ι1) w, fun _ : Assignment w => inst e' ι1) (t, e') ι1).
-      unfold entails, implₚ in RQ. cbn in RQ.
-      rewrite inst_persist_ty, inst_lift in RQ.
-      specialize (RQ eq_refl). intuition.
-    - intros (t & e' & HT & HQ).
-      generalize (@completeness_aux e w G ι (inst G ι) eq_refl (inst t ι) (inst e' ι) HT).
-      apply wp_monotonic. intros w1 r01 [t1 e1'] ι1 (Heq & Heqt). subst.
-      specialize (RQ _ r01 (t,e') (t1,e1') ι1). cbn in RQ.
-      rewrite inst_persist_ty, Heqt in RQ.
-      apply RQ; auto. f_equal. clear.
-      admit.
-  Admitted.
-
-End Correctness.
-
-Section WithPredicates.
-
-  Import World.notations.
-  Import Pred Pred.notations.
-  Import (hints) Pred Pred.Acc.
-
-  Definition WP {A} : ⊢ FreeM A -> □⁺(A -> Pred) -> Pred :=
-    fix WP (w : World) (m : FreeM A w) (POST : □⁺(A -> Pred) w) {struct m} :=
-      match m with
-      | Ret_Free _ _ v => T POST v
-      | Fail_Free _ _ => ⊥ₚ%P
-      | Bind_AssertEq_Free _ _ t1 t2 k => (t1 =ₚ t2 /\ₚ WP w k POST)%P
-      | Bind_Exists_Free _ _ i k =>
-          Acc.wp step (WP (w ▻ i) k (fun w1 r01 => _4 POST step r01))
-      end.
-
-  Definition WLP {A} : ⊢ FreeM A -> □⁺(A -> Pred) -> Pred :=
-    fix WLP (w : World) (m : FreeM A w) (POST : □⁺(A -> Pred) w) {struct m} :=
-      match m with
-      | Ret_Free _ _ v => T POST v
-      | Fail_Free _ _ => ⊤ₚ%P
-      | Bind_AssertEq_Free _ _ t1 t2 k => (t1 =ₚ t2 ->ₚ WLP w k POST)%P
-      | Bind_Exists_Free _ _ i k =>
-          Acc.wlp step (WLP (w ▻ i) k (fun w1 r01 => _4 POST step r01))
-      end.
-
-  Lemma wp_bind {A B w1} (m : FreeM A w1) (f : □⁺(A -> FreeM B) w1) :
-    forall (Q : □⁺(B -> Pred) w1),
-      WP w1 (bind m f) Q ⊣⊢ₚ
-      WP w1 m (fun w1 r01 a => WP w1 (f _ r01 a) (_4 Q r01)).
-  Proof. split; intros; induction m; cbn; firstorder; exists x; firstorder. Qed.
-
-  Lemma wlp_bind {A B w1} (m : FreeM A w1) (f : □⁺(A -> FreeM B) w1) :
-    forall (Q : □⁺(B -> Pred) w1),
-      WLP w1 (bind m f) Q ⊣⊢ₚ
-      WLP w1 m (fun w1 r01 a => WLP w1 (f _ r01 a) (_4 Q r01)).
-  Proof. split; intros; induction m; cbn; firstorder; exists x; firstorder. Qed.
-
-  Lemma wp_monotonic' {A w} (m : FreeM A w) (R : Pred w) (P Q : □⁺(A -> Pred) w) :
-    (forall w1 (r : Alloc w w1) (a : A w1),
-        Ext R r ⊢ₚ P w1 r a ->ₚ Q w1 r a) ->
-    R ⊢ₚ WP w m P ->ₚ WP w m Q.
-  Proof. Admitted.
-
-  Lemma wlp_monotonic' {A w} (m : FreeM A w) (R : Pred w) (P Q : □⁺(A -> Pred) w) :
-    (forall w1 (r : Alloc w w1) (a : A w1),
-        Ext R r ⊢ₚ P w1 r a ->ₚ Q w1 r a) ->
-    R ⊢ₚ WLP w m P ->ₚ WLP w m Q.
-  Proof.
-    intros pq. destruct m; cbn.
-    - specialize (pq w refl a). rewrite ext_refl in pq. apply pq.
-    - apply impl_and_adjoint. apply true_r.
-    - admit.
-    - apply impl_and_adjoint. admit.
-  Admitted.
-
-  Lemma wp_frame2 {A w} (m : FreeM A w) (P : □⁺(A -> Pred) w) (Q : Pred w) :
-    WP w m P /\ₚ Q ⊣⊢ₚ WP w m (fun _ θ a => P _ θ a /\ₚ Ext Q θ)%P.
-  Proof. Admitted.
-
-  Lemma completeness e : forall (w0 : World) (G : Env w0) {t ee},
-    (TPB G e t ee)
-    ⊢ₚ
-    WP w0 (reconstruct e G)
-        (fun w1 r01 '(t', ee') => (<{ ee ~ r01 }> =ₚ ee' /\ₚ <{ t ~ r01 }> =ₚ t')%P).
-  Proof.
-    intros. revert w0 G e t ee. apply TPB_ind; cbn.
-    - intro w.
-      apply forall_r. intros _.
-      apply forall_r. intros t.
-      apply forall_r. intros ee ι.
-      unfold T. cbn. intros _ Ht Hee.
-      now rewrite inst_persist_ty, inst_refl.
-    - intro w.
-      apply forall_r. intros _.
-      apply forall_r. intros t.
-      apply forall_r. intros ee ι.
-      unfold T. cbn. intros _ Ht Hee.
-      now rewrite inst_persist_ty, inst_refl.
-    - intro w1.
-      do 9 (apply forall_r; intros ?).
-      do 7 (rewrite <- impl_and_adjoint).
-      assert (MASSAGE: forall w (A B C D E F G : Pred w),
-  bientails (andₚ (andₚ (andₚ (andₚ (andₚ (andₚ A B) C) D) E) F) G)
-            (andₚ (andₚ (andₚ (andₚ (andₚ (andₚ A B) C) G) E) F) D)) by admit.
-      rewrite MASSAGE. clear MASSAGE.
-      rewrite wp_bind. apply impl_and_adjoint. apply wp_monotonic'.
-      intros w2 r12 [t1 ee1]. cbn -[step]. unfold Definitions.T, _4.
-      rewrite wp_bind.
-      rewrite <- impl_and_adjoint.
-      rewrite (eqₚ_sym t1).
-      assert (MASSAGE: forall w (A B C D : Pred w),
-                 entails (andₚ A (andₚ B C)) (andₚ C D) <-> entails (andₚ A (andₚ B ⊤ₚ)) D) by admit.
-      rewrite (MASSAGE _ _ (eqₚ (persist w1 x4 w2 r12) ee1) (eqₚ (Ty_bool w2) t1) _).
-      rewrite and_true_r.
-      admit.
-    - intros w G s t e' ι. cbn.
-      intros _ Heqo Hvar. destruct (resolve s G) eqn:?; cbn; inversion Heqo.
-      unfold T. firstorder. now rewrite refl_persist.
-    - admit.
-    - admit.
-    - admit.
-  Admitted.
-
-  Lemma soundness' e : forall (w0 : World) (G : Env w0),
-    Trueₚ
-    ⊢ₚ
-    WLP w0 (reconstruct e G)
-        (fun w1 r01 '(t, ee) => TPB <{G ~ r01}> e t ee).
-  Proof.
-    Set Printing Depth 20.
-    induction e; cbn; intros; subst; try constructor.
-    - rewrite wlp_bind. rewrite IHe1.
-      rewrite <- and_true_l. apply impl_and_adjoint. apply wlp_monotonic'.
-      intros. rewrite ext_true.
-      destruct a. rewrite <- impl_and_adjoint.
-      cbn. rewrite <- impl_and_adjoint. unfold T. rewrite wlp_bind.
-      specialize (IHe2 w1 <{ G ~ r ⊙ refl }>). rewrite IHe2.
-      (* probably doable with some kind of tactic, perhaps change or replace X with Y is easier? *)
-      assert (MASSAGE: forall w (X Y Z : Pred w), bientails (andₚ (andₚ X Y) Z) (andₚ (andₚ Y Z) X)).
-      { intros. now rewrite (and_assoc X _), (and_comm _ X). }
-      rewrite MASSAGE. clear MASSAGE.
-      apply impl_and_adjoint. apply wlp_monotonic'.
-      intros. destruct a. rewrite wlp_bind.
-      rewrite <- impl_and_adjoint. rewrite <- and_true_r.
-      rewrite IHe3.
-      apply impl_and_adjoint. apply wlp_monotonic'.
-      intros. destruct a. cbn. unfold T, _4. clear.
-      rewrite trans_refl_r, trans_refl_r.
-      intro. unfold Ext. unfold andₚ, implₚ, TPB. intros.
-      destruct H as [[]].
-      constructor.
-      + rewrite inst_persist_env, ?inst_trans.
-        rewrite inst_persist_env, H2 in H. cbn in H.
-        rewrite persist_trans.
-        exact H.
-      + rewrite inst_persist_env, inst_trans, inst_trans, inst_persist_ty.
-        rewrite inst_persist_env, inst_persist_env in H3.
-        apply H3.
-      + rewrite inst_persist_env, inst_trans, inst_trans.
-        rewrite inst_persist_env, inst_persist_env, inst_trans, <- H1 in H0.
-        apply H0.
-    - destruct (resolve s G) eqn:?; cbn; try easy.
-      unfold T. rewrite refl_persist. constructor.
-      now rewrite resolve_inst, Heqo.
-    - rewrite <- Acc.entails_wlp. rewrite ext_true. rewrite IHe.
-      rewrite <- and_true_l.
-      apply impl_and_adjoint. unfold T, _4. rewrite wlp_bind.
-      apply wlp_monotonic'.
-      intros. rewrite ext_true.
-      destruct a. cbn -[step]. unfold T, _4.
-      rewrite trans_refl_r, trans_refl_r.
-      intro. cbn -[step].
-      unfold Ext, andₚ, implₚ, TPB. intros. cbn -[step] in *.
-      constructor. rewrite ?inst_persist_env in *. exact H0.
-    - rewrite wlp_bind. specialize (IHe w0 ((s, lift t w0) :: G)). rewrite IHe.
-      rewrite <- and_true_l.
-      apply impl_and_adjoint.
-      apply wlp_monotonic'.
-      intros. rewrite ext_true. destruct a. rewrite <- impl_and_adjoint.
-      rewrite and_true_l. cbn in *. unfold T, _4.
-      intros ι He. cbn in *. rewrite ?inst_persist_env, ?inst_persist_ty, ?trans_refl_r, ?inst_lift in *. now constructor.
-
-
-    - rewrite <- Acc.entails_wlp, ext_true, IHe2, <- and_true_l.
-      apply impl_and_adjoint. unfold T, _4. rewrite wlp_bind. apply wlp_monotonic'.
-      intros w1 r [t2 e2'].
-      rewrite ext_true, wlp_bind, <- impl_and_adjoint, and_comm, IHe1.
-      apply impl_and_adjoint. apply wlp_monotonic'.
-      intros w2 r12 [t1 e1']. cbn -[step]. unfold T, _4.
-      rewrite ?trans_refl_r.
-      unfold Ext, eqₚ, TPB, entails.
-      cbn -[step] in *.
-      intros ι He2 He1 Ht1.
-      rewrite ?inst_persist_ty, ?inst_persist_env, ?inst_trans, ?assoc_persist in *.
-      rewrite Ht1 in He1. econstructor.
-      exact He1. exact He2.
-  Qed.
-
-End WithPredicates.
